07TreeCode/TreeCodeConversion.thy
@@ -1,49 +1,49 @@
 theory TreeCodeConversion
-  imports TreeCode "../05Closure/Closure" "../03Debruijn/LetFloating"
+  imports TreeCode "../06GroupedEnvironments/GroupedEnvironments"
 begin
 
 subsection \<open>Compilation to Tree-Code\<close>
 
-text \<open>This is our first real compilation phase; typechecking and name-removal were fundamentally 
-just modifying an underlying expression, but here we genuinely reshape our expressions into code. 
-The first few steps are simple: encoding an expression means shuffling it into a postfix form, and 
-tree-code closures-values are just encoded stack closure-values. We add a \<open>Return\<^sub>e\<close> operation on at 
-the end of every code block, too; we never encode the \<open>Jump\<^sub>e\<close> operation. Its place will come a 
-little later.\<close>
+text \<open>This is our first real compilation phase; typechecking, name-removal, and variable-splitting 
+were fundamentally just modifying an underlying expression, but here we genuinely reshape our 
+expressions into code. The first few steps are simple: encoding an expression means shuffling it 
+into a postfix form, and tree-code closures-values are just encoded stack closure-values. We add a 
+\<open>Return\<^sub>e\<close> operation on at the end of every code block, too; we never encode the \<open>Jump\<^sub>e\<close> operation. 
+Its place will come a little later.\<close>
 
-primrec encode' :: "expr\<^sub>d \<Rightarrow> code\<^sub>e list" where
-  "encode' (Var\<^sub>d x) = [Lookup\<^sub>e x 0 0]"
-| "encode' (Const\<^sub>d n) = [PushCon\<^sub>e n]"
-| "encode' (Lam\<^sub>d t e) = [PushLam\<^sub>e (encode' e @ [Return\<^sub>e]) (length (strip_lets e))]"
-| "encode' (App\<^sub>d e\<^sub>1 e\<^sub>2) = encode' e\<^sub>1 @ encode' e\<^sub>2 @ [Apply\<^sub>e]"
-| "encode' (Let\<^sub>d e\<^sub>1 e\<^sub>2) = encode' e\<^sub>1 @ PushEnv\<^sub>e # encode' e\<^sub>2 @ [PopEnv\<^sub>e]"
+primrec encode' :: "expr\<^sub>g \<Rightarrow> code\<^sub>e list" where
+  "encode' (Var\<^sub>g x y) = [Lookup\<^sub>e x y]"
+| "encode' (Const\<^sub>g n) = [PushCon\<^sub>e n]"
+| "encode' (Lam\<^sub>g t e n) = [PushLam\<^sub>e (encode' e @ [Return\<^sub>e]) n]"
+| "encode' (App\<^sub>g e\<^sub>1 e\<^sub>2) = encode' e\<^sub>1 @ encode' e\<^sub>2 @ [Apply\<^sub>e]"
+| "encode' (Let\<^sub>g e\<^sub>1 e\<^sub>2) = encode' e\<^sub>1 @ PushEnv\<^sub>e # encode' e\<^sub>2 @ [PopEnv\<^sub>e]"
 
-definition encode :: "expr\<^sub>d \<Rightarrow> code\<^sub>e list" where
+definition encode :: "expr\<^sub>g \<Rightarrow> code\<^sub>e list" where
   "encode e \<equiv> encode' e @ [Return\<^sub>e]"
 
-primrec encode_closure :: "closure\<^sub>c \<Rightarrow> closure\<^sub>e" where
-  "encode_closure (Const\<^sub>c n) = Const\<^sub>e n"
-| "encode_closure (Lam\<^sub>c t \<Delta> e) = Lam\<^sub>e (map encode_closure \<Delta>) (encode e)"
+primrec encode_closure :: "closure\<^sub>g \<Rightarrow> closure\<^sub>e" where
+  "encode_closure (Num\<^sub>g n) = Const\<^sub>e n"
+| "encode_closure (Fun\<^sub>g t \<Delta> e n) = Lam\<^sub>e (map (map encode_closure) \<Delta>) (encode e) n" 
 
 lemma tl_encode [simp]: "tl (encode' e @ \<C>) = tl (encode' e) @ \<C>"
   by (induction e arbitrary: \<C>) simp_all
 
 text \<open>It is the callstack where things get complicated: we have to divide the stack into a 
-callstack and a value stack. The value stack consists of the returned closure-values in \<open>FApp2\<^sub>c\<close> 
+callstack and a value stack. The value stack consists of the returned closure-values in \<open>FApp2\<^sub>g\<close> 
 frames:\<close>
 
-fun vals_from_stack :: "frame\<^sub>c list \<Rightarrow> closure\<^sub>e list" where
+fun vals_from_stack :: "frame\<^sub>g list \<Rightarrow> closure\<^sub>e list" where
   "vals_from_stack [] = []"
-| "vals_from_stack (FApp1\<^sub>c \<Delta> e # s\<^sub>c) = vals_from_stack s\<^sub>c"
-| "vals_from_stack (FApp2\<^sub>c c # s\<^sub>c) = encode_closure c # vals_from_stack s\<^sub>c"
-| "vals_from_stack (FLet\<^sub>c \<Delta> e # s\<^sub>c) = vals_from_stack s\<^sub>c"
-| "vals_from_stack (FPop\<^sub>c c # s\<^sub>c) = vals_from_stack s\<^sub>c"
-| "vals_from_stack (FReturn\<^sub>c \<Delta> # s\<^sub>c) = vals_from_stack s\<^sub>c"
+| "vals_from_stack (FApp1\<^sub>g \<Delta> e # s\<^sub>g) = vals_from_stack s\<^sub>g"
+| "vals_from_stack (FApp2\<^sub>g c # s\<^sub>g) = encode_closure c # vals_from_stack s\<^sub>g"
+| "vals_from_stack (FLet\<^sub>g \<Delta> e # s\<^sub>g) = vals_from_stack s\<^sub>g"
+| "vals_from_stack (FPop\<^sub>g c # s\<^sub>g) = vals_from_stack s\<^sub>g"
+| "vals_from_stack (FReturn\<^sub>g \<Delta> # s\<^sub>g) = vals_from_stack s\<^sub>g"
 
 text \<open>The callstack requires some more careful work. Each frame represents a place where we are part
 of the way through the block of code associated with a particular expression; fortunately, we can 
 reconstruct what the code must have been to get us to this state, and then prepend it into the most
-recent stack frame. The \<open>FReturn\<^sub>c\<close> frames and their environments that we have been so diligently 
+recent stack frame. The \<open>FReturn\<^sub>g\<close> frames and their environments that we have been so diligently 
 recording for the last two stages finally prove their worth, as well: they show us where (and with 
 what environment) callstack frames begin.\<close>
 
@@ -53,18 +53,19 @@ fun prepend_to_top_frame :: "code\<^sub>e list \<Rightarrow> frame\<^sub>e list 
 
 fun prepend_to_top_env :: "closure\<^sub>e \<Rightarrow> frame\<^sub>e list \<Rightarrow> frame\<^sub>e list" where
   "prepend_to_top_env c [] = []"
-| "prepend_to_top_env c ((\<Delta>, \<C>) # s\<^sub>e) = (c # \<Delta>, \<C>) # s\<^sub>e"
+| "prepend_to_top_env c ((\<Delta>, \<C>) # s\<^sub>e) = (cons_fst c \<Delta>, \<C>) # s\<^sub>e"
 
-fun stack_from_stack :: "frame\<^sub>c list \<Rightarrow> frame\<^sub>e list" where
+fun stack_from_stack :: "frame\<^sub>g list \<Rightarrow> frame\<^sub>e list" where
   "stack_from_stack [] = []"
-| "stack_from_stack (FApp1\<^sub>c \<Delta> e # s\<^sub>c) = 
-    prepend_to_top_frame (encode' e @ [Apply\<^sub>e]) (stack_from_stack s\<^sub>c)"
-| "stack_from_stack (FApp2\<^sub>c c # s\<^sub>c) = prepend_to_top_frame [Apply\<^sub>e] (stack_from_stack s\<^sub>c)"
-| "stack_from_stack (FLet\<^sub>c \<Delta> e # s\<^sub>c) = 
-    prepend_to_top_frame (PushEnv\<^sub>e # encode' e @ [PopEnv\<^sub>e]) (stack_from_stack s\<^sub>c)"
-| "stack_from_stack (FPop\<^sub>c c # s\<^sub>c) = 
-    prepend_to_top_frame [PopEnv\<^sub>e] (prepend_to_top_env (encode_closure c) (stack_from_stack s\<^sub>c))"
-| "stack_from_stack (FReturn\<^sub>c \<Delta> # s\<^sub>c) = (map encode_closure \<Delta>, [Return\<^sub>e]) # stack_from_stack s\<^sub>c"
+| "stack_from_stack (FApp1\<^sub>g \<Delta> e # s\<^sub>g) = 
+    prepend_to_top_frame (encode' e @ [Apply\<^sub>e]) (stack_from_stack s\<^sub>g)"
+| "stack_from_stack (FApp2\<^sub>g c # s\<^sub>g) = prepend_to_top_frame [Apply\<^sub>e] (stack_from_stack s\<^sub>g)"
+| "stack_from_stack (FLet\<^sub>g \<Delta> e # s\<^sub>g) = 
+    prepend_to_top_frame (PushEnv\<^sub>e # encode' e @ [PopEnv\<^sub>e]) (stack_from_stack s\<^sub>g)"
+| "stack_from_stack (FPop\<^sub>g c # s\<^sub>g) = 
+    prepend_to_top_frame [PopEnv\<^sub>e] (prepend_to_top_env (encode_closure c) (stack_from_stack s\<^sub>g))"
+| "stack_from_stack (FReturn\<^sub>g \<Delta> # s\<^sub>g) = 
+    (map (map encode_closure) \<Delta>, [Return\<^sub>e]) # stack_from_stack s\<^sub>g"
 
 lemma prepend_nil [simp]: "prepend_to_top_frame [] s\<^sub>e = s\<^sub>e"
   by (induction "[] :: code\<^sub>e list" s\<^sub>e rule: prepend_to_top_frame.induct) simp_all
@@ -77,97 +78,99 @@ text \<open>We once again collapse the distinction between our two states, evalu
 evaluation state is simply one where a little more code is there to be executed in the topmost 
 frame.\<close>
 
-primrec encode_state :: "state\<^sub>c \<Rightarrow> state\<^sub>e" where
-  "encode_state (SE\<^sub>c s\<^sub>c \<Delta> e) = 
-    S\<^sub>e (vals_from_stack s\<^sub>c) (prepend_to_top_frame (encode' e) (stack_from_stack s\<^sub>c))"
-| "encode_state (SC\<^sub>c s\<^sub>c c) = S\<^sub>e (encode_closure c # vals_from_stack s\<^sub>c) (stack_from_stack s\<^sub>c)"
+primrec encode_state :: "state\<^sub>g \<Rightarrow> state\<^sub>e" where
+  "encode_state (SE\<^sub>g s\<^sub>g \<Delta> e) = 
+    S\<^sub>e (vals_from_stack s\<^sub>g) (prepend_to_top_frame (encode' e) (stack_from_stack s\<^sub>g))"
+| "encode_state (SC\<^sub>g s\<^sub>g c) = S\<^sub>e (encode_closure c # vals_from_stack s\<^sub>g) (stack_from_stack s\<^sub>g)"
 
 text \<open>Because the conversion functions run forwards, we can once again prove correctness easily.
 (Because we have no typing judgement for tree code, we do not - cannot - prove type safety.) 
 We again have to use \<open>iter\<close> in our statement of the theorem, because the frame-adjustment evaluation
-steps (\<open>ret\<^sub>c_app1\<close> and \<open>ret\<^sub>c_app2\<close>) are not matched by any steps in the tree-code evaluation.\<close>
+steps (\<open>ret\<^sub>g_app1\<close> and \<open>ret\<^sub>g_app2\<close>) are not matched by any steps in the tree-code evaluation.\<close>
 
-lemma lookup_latest [dest]: "latest_environment\<^sub>c s\<^sub>c = Some \<Delta> \<Longrightarrow> 
-    \<exists>\<C> s\<^sub>e. stack_from_stack s\<^sub>c = (map encode_closure \<Delta>, \<C>) # s\<^sub>e"
-  by (induction s\<^sub>c arbitrary: \<Delta> rule: stack_from_stack.induct) fastforce+
+lemma lookup_latest [dest]: "latest_environment\<^sub>g s\<^sub>g = Some \<Delta> \<Longrightarrow> 
+    \<exists>\<C> s\<^sub>e. stack_from_stack s\<^sub>g = (map (map encode_closure) \<Delta>, \<C>) # s\<^sub>e"
+  by (induction s\<^sub>g arbitrary: \<Delta> rule: stack_from_stack.induct) fastforce+
 
-theorem correct\<^sub>e [simp]: "\<Sigma> \<leadsto>\<^sub>c \<Sigma>' \<Longrightarrow> \<Sigma> :\<^sub>c t \<Longrightarrow> iter (\<leadsto>\<^sub>e) (encode_state \<Sigma>) (encode_state \<Sigma>')"
-proof (induction \<Sigma> \<Sigma>' rule: eval\<^sub>c.induct)
-  case (ev\<^sub>c_var \<Delta> x c s\<^sub>c)
-  then obtain t' \<Gamma> where "(s\<^sub>c :\<^sub>c t' \<rightarrow> t) \<and> (\<Delta> :\<^sub>c\<^sub>l\<^sub>s \<Gamma>) \<and> latest_environment\<^sub>c s\<^sub>c = Some \<Delta> \<and> 
-    lookup \<Gamma> x = Some t'" by fastforce
-  then obtain \<C> s\<^sub>e where S: "stack_from_stack s\<^sub>c = (map encode_closure \<Delta>, \<C>) # s\<^sub>e" by auto
-  with ev\<^sub>c_var have "S\<^sub>e (vals_from_stack s\<^sub>c) ((map encode_closure \<Delta>, Lookup\<^sub>e x 0 0 # \<C>) # s\<^sub>e) \<leadsto>\<^sub>e 
-    S\<^sub>e (encode_closure c # vals_from_stack s\<^sub>c) ((map encode_closure \<Delta>, \<C>) # s\<^sub>e)" by simp
-  hence "iter (\<leadsto>\<^sub>e) (S\<^sub>e (vals_from_stack s\<^sub>c) ((map encode_closure \<Delta>, Lookup\<^sub>e x 0 0 # \<C>) # s\<^sub>e))
-    (S\<^sub>e (encode_closure c # vals_from_stack s\<^sub>c) ((map encode_closure \<Delta>, \<C>) # s\<^sub>e))" 
+theorem correct\<^sub>e [simp]: "\<Sigma> \<leadsto>\<^sub>g \<Sigma>' \<Longrightarrow> \<Sigma> :\<^sub>g t \<Longrightarrow> iter (\<leadsto>\<^sub>e) (encode_state \<Sigma>) (encode_state \<Sigma>')"
+proof (induction \<Sigma> \<Sigma>' rule: eval\<^sub>g.induct)
+  case (ev\<^sub>g_var \<Delta> x ts y c s\<^sub>g)
+  then obtain ts t' \<Gamma> where "(s\<^sub>g :\<^sub>g t' \<rightarrow> t) \<and> (\<Delta> :\<^sub>g\<^sub>c\<^sub>l\<^sub>s \<Gamma>) \<and> latest_environment\<^sub>g s\<^sub>g = Some \<Delta> \<and> 
+    lookup \<Gamma> x = Some ts \<and> lookup ts y = Some t'" by fastforce
+  then obtain \<C> s\<^sub>e where S: "stack_from_stack s\<^sub>g = (map (map encode_closure) \<Delta>, \<C>) # s\<^sub>e" by auto
+  with ev\<^sub>g_var have "
+    S\<^sub>e (vals_from_stack s\<^sub>g) ((map (map encode_closure) \<Delta>, Lookup\<^sub>e x y # \<C>) # s\<^sub>e) \<leadsto>\<^sub>e 
+      S\<^sub>e (encode_closure c # vals_from_stack s\<^sub>g) ((map (map encode_closure) \<Delta>, \<C>) # s\<^sub>e)" by simp
+  hence "iter (\<leadsto>\<^sub>e) (S\<^sub>e (vals_from_stack s\<^sub>g) ((map (map encode_closure) \<Delta>, Lookup\<^sub>e x y # \<C>) # s\<^sub>e))
+    (S\<^sub>e (encode_closure c # vals_from_stack s\<^sub>g) ((map (map encode_closure) \<Delta>, \<C>) # s\<^sub>e))" 
       by (metis iter_one)
   with S show ?case by simp
 next
-  case (ev\<^sub>c_con s\<^sub>c \<Delta> n)
-  then obtain \<Gamma> where "(s\<^sub>c :\<^sub>c Num \<rightarrow> t) \<and> (\<Delta> :\<^sub>c\<^sub>l\<^sub>s \<Gamma>) \<and> latest_environment\<^sub>c s\<^sub>c = Some \<Delta>" by fastforce
-  then obtain \<C> s\<^sub>e where S: "stack_from_stack s\<^sub>c = (map encode_closure \<Delta>, \<C>) # s\<^sub>e" by auto
-  have "iter (\<leadsto>\<^sub>e) (S\<^sub>e (vals_from_stack s\<^sub>c) ((map encode_closure \<Delta>, PushCon\<^sub>e n # \<C>) # s\<^sub>e)) 
-    (S\<^sub>e (Const\<^sub>e n # vals_from_stack s\<^sub>c) ((map encode_closure \<Delta>, \<C>) # s\<^sub>e))" 
+  case (ev\<^sub>g_con s\<^sub>g \<Delta> n)
+  then obtain \<Gamma> where "(s\<^sub>g :\<^sub>g Num \<rightarrow> t) \<and> (\<Delta> :\<^sub>g\<^sub>c\<^sub>l\<^sub>s \<Gamma>) \<and> latest_environment\<^sub>g s\<^sub>g = Some \<Delta>" 
+    by fastforce
+  then obtain \<C> s\<^sub>e where S: "stack_from_stack s\<^sub>g = (map (map encode_closure) \<Delta>, \<C>) # s\<^sub>e" by auto
+  have "iter (\<leadsto>\<^sub>e) (S\<^sub>e (vals_from_stack s\<^sub>g) ((map (map encode_closure) \<Delta>, PushCon\<^sub>e n # \<C>) # s\<^sub>e)) 
+    (S\<^sub>e (Const\<^sub>e n # vals_from_stack s\<^sub>g) ((map (map encode_closure) \<Delta>, \<C>) # s\<^sub>e))" 
       by (metis ev\<^sub>e_pushcon iter_one)
   with S show ?case by simp
 next
-  case (ev\<^sub>c_lam s\<^sub>c \<Delta> tt e)
-  then obtain t' \<Gamma> where "(s\<^sub>c :\<^sub>c t' \<rightarrow> t) \<and> (\<Delta> :\<^sub>c\<^sub>l\<^sub>s \<Gamma>) \<and> latest_environment\<^sub>c s\<^sub>c = Some \<Delta> \<and>
-    (\<Gamma> \<turnstile>\<^sub>d Lam\<^sub>d tt e : t')" by fastforce
-  then obtain \<C> s\<^sub>e where S: "stack_from_stack s\<^sub>c = (map encode_closure \<Delta>, \<C>) # s\<^sub>e" by auto
-  have "iter (\<leadsto>\<^sub>e) (S\<^sub>e (vals_from_stack s\<^sub>c) 
-    ((map encode_closure \<Delta>, PushLam\<^sub>e (encode e) (length (strip_lets e)) # \<C>) # s\<^sub>e)) 
-      (S\<^sub>e (Lam\<^sub>e (map encode_closure \<Delta>) (encode e) # vals_from_stack s\<^sub>c)
-        ((map encode_closure \<Delta>, \<C>) # s\<^sub>e))" by (metis ev\<^sub>e_pushlam iter_one)
+  case (ev\<^sub>g_lam s\<^sub>g \<Delta> tt e n)
+  then obtain t' \<Gamma> where "(s\<^sub>g :\<^sub>g t' \<rightarrow> t) \<and> (\<Delta> :\<^sub>g\<^sub>c\<^sub>l\<^sub>s \<Gamma>) \<and> latest_environment\<^sub>g s\<^sub>g = Some \<Delta> \<and>
+    (\<Gamma> \<turnstile>\<^sub>g Lam\<^sub>g tt e n : t')" by fastforce
+  then obtain \<C> s\<^sub>e where S: "stack_from_stack s\<^sub>g = (map (map encode_closure) \<Delta>, \<C>) # s\<^sub>e" by auto
+  have "iter (\<leadsto>\<^sub>e) (S\<^sub>e (vals_from_stack s\<^sub>g) ((map (map encode_closure) \<Delta>, 
+    PushLam\<^sub>e (encode e) n # \<C>) # s\<^sub>e)) 
+      (S\<^sub>e (Lam\<^sub>e (map (map encode_closure) \<Delta>) (encode e) n # vals_from_stack s\<^sub>g)
+        ((map (map encode_closure) \<Delta>, \<C>) # s\<^sub>e))" by (metis ev\<^sub>e_pushlam iter_one)
   with S show ?case by (simp add: encode_def)
 next
-  case (ret\<^sub>c_app2 t\<^sub>1 \<Delta> e\<^sub>1 s\<^sub>c c\<^sub>2)
-  then obtain \<Gamma> t\<^sub>2 \<Delta>' where "(\<Delta> :\<^sub>c\<^sub>l\<^sub>s \<Gamma>) \<and> (insert_at 0 t\<^sub>1 \<Gamma> \<turnstile>\<^sub>d e\<^sub>1 : t\<^sub>2) \<and> (s\<^sub>c :\<^sub>c t\<^sub>2 \<rightarrow> t) \<and> 
-    latest_environment\<^sub>c s\<^sub>c = Some \<Delta>' \<and> (c\<^sub>2 :\<^sub>c\<^sub>l t\<^sub>1)" by blast
-  then obtain \<C> s\<^sub>e where S: "stack_from_stack s\<^sub>c = (map encode_closure \<Delta>', \<C>) # s\<^sub>e" by auto
+  case (ret\<^sub>g_app2 t\<^sub>1 \<Delta> e\<^sub>1 n s\<^sub>g c\<^sub>2)
+  then obtain \<Gamma> t\<^sub>2 \<Delta>' where "(\<Delta> :\<^sub>g\<^sub>c\<^sub>l\<^sub>s \<Gamma>) \<and> (insert_at 0 [t\<^sub>1] \<Gamma> \<turnstile>\<^sub>g e\<^sub>1 : t\<^sub>2) \<and> (s\<^sub>g :\<^sub>g t\<^sub>2 \<rightarrow> t) \<and> 
+    latest_environment\<^sub>g s\<^sub>g = Some \<Delta>' \<and> (c\<^sub>2 :\<^sub>g\<^sub>c\<^sub>l t\<^sub>1)" by blast
+  then obtain \<C> s\<^sub>e where S: "stack_from_stack s\<^sub>g = (map (map encode_closure) \<Delta>', \<C>) # s\<^sub>e" by auto
   hence "iter (\<leadsto>\<^sub>e) 
-    (S\<^sub>e (encode_closure c\<^sub>2 # Lam\<^sub>e (map encode_closure \<Delta>) (encode e\<^sub>1) # vals_from_stack s\<^sub>c) 
-      ((map encode_closure \<Delta>', Apply\<^sub>e # \<C>) # s\<^sub>e)) 
-    (S\<^sub>e (vals_from_stack s\<^sub>c) ((encode_closure c\<^sub>2 # map encode_closure \<Delta>, encode e\<^sub>1) # 
-      stack_from_stack s\<^sub>c))" by (metis ev\<^sub>e_apply iter_one)
+    (S\<^sub>e (encode_closure c\<^sub>2 # Lam\<^sub>e (map (map encode_closure) \<Delta>) (encode e\<^sub>1) n # vals_from_stack s\<^sub>g) 
+      ((map (map encode_closure) \<Delta>', Apply\<^sub>e # \<C>) # s\<^sub>e)) 
+    (S\<^sub>e (vals_from_stack s\<^sub>g) (([encode_closure c\<^sub>2] # map (map encode_closure) \<Delta>, encode e\<^sub>1) # 
+      stack_from_stack s\<^sub>g))" by (metis ev\<^sub>e_apply iter_one)
   with S show ?case by (simp add: encode_def)
 next
-  case (ret\<^sub>c_let \<Delta> e\<^sub>2 s\<^sub>c c\<^sub>1)
-  then obtain \<Gamma> t\<^sub>1 t\<^sub>2 where "latest_environment\<^sub>c s\<^sub>c = Some \<Delta> \<and> (\<Delta> :\<^sub>c\<^sub>l\<^sub>s \<Gamma>) \<and> 
-    (insert_at 0 t\<^sub>1 \<Gamma> \<turnstile>\<^sub>d e\<^sub>2 : t\<^sub>2) \<and> (s\<^sub>c :\<^sub>c t\<^sub>2 \<rightarrow> t) \<and> (c\<^sub>1 :\<^sub>c\<^sub>l t\<^sub>1)" by blast
-  then obtain \<C> s\<^sub>e where S: "stack_from_stack s\<^sub>c = (map encode_closure \<Delta>, \<C>) # s\<^sub>e" by auto
+  case (ret\<^sub>g_let \<Delta> e\<^sub>2 s\<^sub>g c\<^sub>1)
+  then obtain \<Gamma> t\<^sub>1 t\<^sub>2 where "latest_environment\<^sub>g s\<^sub>g = Some \<Delta> \<and> (\<Delta> :\<^sub>g\<^sub>c\<^sub>l\<^sub>s \<Gamma>) \<and> 
+    (cons_fst t\<^sub>1 \<Gamma> \<turnstile>\<^sub>g e\<^sub>2 : t\<^sub>2) \<and> (s\<^sub>g :\<^sub>g t\<^sub>2 \<rightarrow> t) \<and> (c\<^sub>1 :\<^sub>g\<^sub>c\<^sub>l t\<^sub>1)" by blast
+  then obtain \<C> s\<^sub>e where S: "stack_from_stack s\<^sub>g = (map (map encode_closure) \<Delta>, \<C>) # s\<^sub>e" by auto
   have "iter (\<leadsto>\<^sub>e)
-    (S\<^sub>e (encode_closure c\<^sub>1 # vals_from_stack s\<^sub>c)
-      ((map encode_closure \<Delta>, PushEnv\<^sub>e # encode' e\<^sub>2 @ PopEnv\<^sub>e # \<C>) # s\<^sub>e))
-    (S\<^sub>e (vals_from_stack s\<^sub>c)
-      ((encode_closure c\<^sub>1 # map encode_closure \<Delta>, encode' e\<^sub>2 @ PopEnv\<^sub>e # \<C>) # s\<^sub>e))" 
+    (S\<^sub>e (encode_closure c\<^sub>1 # vals_from_stack s\<^sub>g)
+      ((map (map encode_closure) \<Delta>, PushEnv\<^sub>e # encode' e\<^sub>2 @ PopEnv\<^sub>e # \<C>) # s\<^sub>e))
+    (S\<^sub>e (vals_from_stack s\<^sub>g)
+      ((cons_fst (encode_closure c\<^sub>1) (map (map encode_closure) \<Delta>), encode' e\<^sub>2 @ PopEnv\<^sub>e # \<C>) # s\<^sub>e))" 
     by (metis ev\<^sub>e_pushenv iter_one)
   with S show ?case by simp
 next
-  case (ret\<^sub>c_pop c' s\<^sub>c c)
-  then obtain \<Delta> tt t' where "latest_environment\<^sub>c s\<^sub>c = Some \<Delta> \<and> (c' :\<^sub>c\<^sub>l tt) \<and> (s\<^sub>c :\<^sub>c t' \<rightarrow> t) \<and> 
-    (c :\<^sub>c\<^sub>l t')" by fastforce
-  then obtain \<C> s\<^sub>e where S: "stack_from_stack s\<^sub>c = (map encode_closure \<Delta>, \<C>) # s\<^sub>e" by auto
-  have "iter (\<leadsto>\<^sub>e)
-    (S\<^sub>e (encode_closure c # vals_from_stack s\<^sub>c)
-      ((encode_closure c' # map encode_closure \<Delta>, PopEnv\<^sub>e # \<C>) # s\<^sub>e))
-    (S\<^sub>e (encode_closure c # vals_from_stack s\<^sub>c) ((map encode_closure \<Delta>, \<C>) # s\<^sub>e))"
+  case (ret\<^sub>g_pop c' s\<^sub>g c)
+  then obtain \<Delta> tt t' where "latest_environment\<^sub>g s\<^sub>g = Some \<Delta> \<and> (c' :\<^sub>g\<^sub>c\<^sub>l tt) \<and> (s\<^sub>g :\<^sub>g t' \<rightarrow> t) \<and> 
+    (c :\<^sub>g\<^sub>c\<^sub>l t')" by fastforce
+  then obtain \<C> s\<^sub>e where S: "stack_from_stack s\<^sub>g = (map (map encode_closure) \<Delta>, \<C>) # s\<^sub>e" by auto
+  hence "iter (\<leadsto>\<^sub>e)
+    (S\<^sub>e (encode_closure c # vals_from_stack s\<^sub>g)
+      ((cons_fst (encode_closure c') (map (map encode_closure) \<Delta>), PopEnv\<^sub>e # \<C>) # s\<^sub>e))
+    (S\<^sub>e (encode_closure c # vals_from_stack s\<^sub>g) ((map (map encode_closure) \<Delta>, \<C>) # s\<^sub>e))" 
       by (metis ev\<^sub>e_popenv iter_one)
   with S show ?case by simp
 next
-  case (ret\<^sub>c_ret \<Delta> s\<^sub>c c)
-  have "S\<^sub>e (encode_closure c # vals_from_stack s\<^sub>c) ((map encode_closure \<Delta>, [Return\<^sub>e]) # 
-    stack_from_stack s\<^sub>c) \<leadsto>\<^sub>e
-    S\<^sub>e (encode_closure c # vals_from_stack s\<^sub>c) (stack_from_stack s\<^sub>c)" by simp
+  case (ret\<^sub>g_ret \<Delta> s\<^sub>g c)
+  have "S\<^sub>e (encode_closure c # vals_from_stack s\<^sub>g) ((map (map encode_closure) \<Delta>, [Return\<^sub>e]) # 
+    stack_from_stack s\<^sub>g) \<leadsto>\<^sub>e
+    S\<^sub>e (encode_closure c # vals_from_stack s\<^sub>g) (stack_from_stack s\<^sub>g)" by simp
   hence "iter (\<leadsto>\<^sub>e) 
-    (S\<^sub>e (encode_closure c # vals_from_stack s\<^sub>c) ((map encode_closure \<Delta>, [Return\<^sub>e]) # 
-    stack_from_stack s\<^sub>c))
-    (S\<^sub>e (encode_closure c # vals_from_stack s\<^sub>c) (stack_from_stack s\<^sub>c))" by (metis iter_one)
+    (S\<^sub>e (encode_closure c # vals_from_stack s\<^sub>g) ((map (map encode_closure) \<Delta>, [Return\<^sub>e]) # 
+    stack_from_stack s\<^sub>g))
+    (S\<^sub>e (encode_closure c # vals_from_stack s\<^sub>g) (stack_from_stack s\<^sub>g))" by (metis iter_one)
   thus ?case by simp
 qed fastforce+
 
-lemma correct\<^sub>e_iter [simp]: "iter (\<leadsto>\<^sub>c) \<Sigma> \<Sigma>' \<Longrightarrow> \<Sigma> :\<^sub>c t \<Longrightarrow>
+lemma correct\<^sub>e_iter [simp]: "iter (\<leadsto>\<^sub>g) \<Sigma> \<Sigma>' \<Longrightarrow> \<Sigma> :\<^sub>g t \<Longrightarrow>
   iter (\<leadsto>\<^sub>e) (encode_state \<Sigma>) (encode_state \<Sigma>')"
 proof (induction \<Sigma> \<Sigma>' rule: iter.induct)
   case (iter_step \<Sigma> \<Sigma>' \<Sigma>'')
@@ -181,41 +184,41 @@ host of reconstruction lemmas, we also need some helper functions just to precis
 \<open>head_expr\<close> and \<open>tail_expr\<close> pull an expression apart into its leftmost leaf (value or variable) and 
 the closure call-stack that the expression will unwind to.\<close>
 
-primrec head_expr :: "expr\<^sub>d \<Rightarrow> expr\<^sub>d" where
-  "head_expr (Var\<^sub>d x) = Var\<^sub>d x"
-| "head_expr (Const\<^sub>d n) = Const\<^sub>d n"
-| "head_expr (Lam\<^sub>d t e) = Lam\<^sub>d t e"
-| "head_expr (App\<^sub>d e\<^sub>1 e\<^sub>2) = head_expr e\<^sub>1"
-| "head_expr (Let\<^sub>d e\<^sub>1 e\<^sub>2) = head_expr e\<^sub>1"
+primrec head_expr :: "expr\<^sub>g \<Rightarrow> expr\<^sub>g" where
+  "head_expr (Var\<^sub>g x y) = Var\<^sub>g x y"
+| "head_expr (Const\<^sub>g n) = Const\<^sub>g n"
+| "head_expr (Lam\<^sub>g t e n) = Lam\<^sub>g t e n"
+| "head_expr (App\<^sub>g e\<^sub>1 e\<^sub>2) = head_expr e\<^sub>1"
+| "head_expr (Let\<^sub>g e\<^sub>1 e\<^sub>2) = head_expr e\<^sub>1"
 
-primrec tail_expr :: "closure\<^sub>c list \<Rightarrow> expr\<^sub>d \<Rightarrow> frame\<^sub>c list" where
-  "tail_expr \<Delta> (Var\<^sub>d x) = []"
-| "tail_expr \<Delta> (Const\<^sub>d n) = []"
-| "tail_expr \<Delta> (Lam\<^sub>d t e) = []"
-| "tail_expr \<Delta> (App\<^sub>d e\<^sub>1 e\<^sub>2) = tail_expr \<Delta> e\<^sub>1 @ [FApp1\<^sub>c \<Delta> e\<^sub>2]"
-| "tail_expr \<Delta> (Let\<^sub>d e\<^sub>1 e\<^sub>2) = tail_expr \<Delta> e\<^sub>1 @ [FLet\<^sub>c \<Delta> e\<^sub>2]"
+primrec tail_expr :: "closure\<^sub>g list list \<Rightarrow> expr\<^sub>g \<Rightarrow> frame\<^sub>g list" where
+  "tail_expr \<Delta> (Var\<^sub>g x y) = []"
+| "tail_expr \<Delta> (Const\<^sub>g n) = []"
+| "tail_expr \<Delta> (Lam\<^sub>g t e n) = []"
+| "tail_expr \<Delta> (App\<^sub>g e\<^sub>1 e\<^sub>2) = tail_expr \<Delta> e\<^sub>1 @ [FApp1\<^sub>g \<Delta> e\<^sub>2]"
+| "tail_expr \<Delta> (Let\<^sub>g e\<^sub>1 e\<^sub>2) = tail_expr \<Delta> e\<^sub>1 @ [FLet\<^sub>g \<Delta> e\<^sub>2]"
 
-lemma vals_from_tail_expr [simp]: "vals_from_stack (tail_expr \<Delta> e @ s\<^sub>c) = vals_from_stack s\<^sub>c"
-  by (induction e arbitrary: s\<^sub>c) simp_all
+lemma vals_from_tail_expr [simp]: "vals_from_stack (tail_expr \<Delta> e @ s\<^sub>g) = vals_from_stack s\<^sub>g"
+  by (induction e arbitrary: s\<^sub>g) simp_all
 
-lemma stack_from_tail_expr [simp]: "stack_from_stack (tail_expr \<Delta> e @ s\<^sub>c) = 
-    prepend_to_top_frame (tl (encode' e)) (stack_from_stack s\<^sub>c)"
-  by (induction e arbitrary: s\<^sub>c) simp_all
+lemma stack_from_tail_expr [simp]: "stack_from_stack (tail_expr \<Delta> e @ s\<^sub>g) = 
+    prepend_to_top_frame (tl (encode' e)) (stack_from_stack s\<^sub>g)"
+  by (induction e arbitrary: s\<^sub>g) simp_all
 
 lemma evaluate_to_head_tail [simp]: "
-  iter (\<leadsto>\<^sub>c) (SE\<^sub>c s \<Delta> e) (SE\<^sub>c (tail_expr \<Delta> e @ s) \<Delta> (head_expr e))"
+  iter (\<leadsto>\<^sub>g) (SE\<^sub>g s \<Delta> e) (SE\<^sub>g (tail_expr \<Delta> e @ s) \<Delta> (head_expr e))"
 proof (induction e arbitrary: s)
-  case (App\<^sub>d e\<^sub>1 e\<^sub>2)
-  moreover have "SE\<^sub>c s \<Delta> (App\<^sub>d e\<^sub>1 e\<^sub>2) \<leadsto>\<^sub>c SE\<^sub>c (FApp1\<^sub>c \<Delta> e\<^sub>2 # s) \<Delta> e\<^sub>1" by simp
-  ultimately have "iter (\<leadsto>\<^sub>c) (SE\<^sub>c s \<Delta> (App\<^sub>d e\<^sub>1 e\<^sub>2))
-    (SE\<^sub>c (tail_expr \<Delta> e\<^sub>1 @ FApp1\<^sub>c \<Delta> e\<^sub>2 # s) \<Delta> (head_expr e\<^sub>1))" 
+  case (App\<^sub>g e\<^sub>1 e\<^sub>2)
+  moreover have "SE\<^sub>g s \<Delta> (App\<^sub>g e\<^sub>1 e\<^sub>2) \<leadsto>\<^sub>g SE\<^sub>g (FApp1\<^sub>g \<Delta> e\<^sub>2 # s) \<Delta> e\<^sub>1" by simp
+  ultimately have "iter (\<leadsto>\<^sub>g) (SE\<^sub>g s \<Delta> (App\<^sub>g e\<^sub>1 e\<^sub>2))
+    (SE\<^sub>g (tail_expr \<Delta> e\<^sub>1 @ FApp1\<^sub>g \<Delta> e\<^sub>2 # s) \<Delta> (head_expr e\<^sub>1))" 
       by (metis iter_step)
     thus ?case by simp
 next
-  case (Let\<^sub>d e1 e2)
-  moreover have "SE\<^sub>c s \<Delta> (Let\<^sub>d e1 e2) \<leadsto>\<^sub>c SE\<^sub>c (FLet\<^sub>c \<Delta> e2 # s) \<Delta> e1" by simp
-  ultimately have "iter (\<leadsto>\<^sub>c) (SE\<^sub>c s \<Delta> (Let\<^sub>d e1 e2)) 
-    (SE\<^sub>c (tail_expr \<Delta> e1 @ FLet\<^sub>c \<Delta> e2 # s) \<Delta> (head_expr e1))" by (metis iter_step)
+  case (Let\<^sub>g e1 e2)
+  moreover have "SE\<^sub>g s \<Delta> (Let\<^sub>g e1 e2) \<leadsto>\<^sub>g SE\<^sub>g (FLet\<^sub>g \<Delta> e2 # s) \<Delta> e1" by simp
+  ultimately have "iter (\<leadsto>\<^sub>g) (SE\<^sub>g s \<Delta> (Let\<^sub>g e1 e2)) 
+    (SE\<^sub>g (tail_expr \<Delta> e1 @ FLet\<^sub>g \<Delta> e2 # s) \<Delta> (head_expr e1))" by (metis iter_step)
   then show ?case by simp
 qed simp_all
 
@@ -227,17 +230,16 @@ lemma encode'_not_nil [simp]: "encode' e \<noteq> []"
 lemma encode_not_nil [simp]: "encode e \<noteq> []"
   by (simp add: encode_def)
 
-lemma encode_to_lookup [dest]: "encode' e @ \<C>' = Lookup\<^sub>e x y z # \<C> \<Longrightarrow> 
-    head_expr e = Var\<^sub>d x \<and> \<C> = tl (encode' e) @ \<C>' \<and> y = 0 \<and> z = 0"
+lemma encode_to_lookup [dest]: "encode' e @ \<C>' = Lookup\<^sub>e x y # \<C> \<Longrightarrow> 
+    head_expr e = Var\<^sub>g x y \<and> \<C> = tl (encode' e) @ \<C>'"
   by (induction e arbitrary: \<C>') fastforce+
 
 lemma encode_to_pushcon [dest]: "encode' e @ \<C>' = PushCon\<^sub>e n # \<C> \<Longrightarrow> 
-    head_expr e = Const\<^sub>d n \<and> \<C> = tl (encode' e) @ \<C>'"
+    head_expr e = Const\<^sub>g n \<and> \<C> = tl (encode' e) @ \<C>'"
   by (induction e arbitrary: \<C>') fastforce+
 
 lemma encode_to_pushlam [dest]: "encode' e @ \<C>' = PushLam\<^sub>e \<C>'' n # \<C> \<Longrightarrow> 
-  \<exists>t e'. head_expr e = Lam\<^sub>d t e' \<and> \<C>'' = encode e' \<and> \<C> = tl (encode' e) @ \<C>' \<and> 
-    n = length (strip_lets e')"
+  \<exists>t e'. head_expr e = Lam\<^sub>g t e' n \<and> \<C>'' = encode e' \<and> \<C> = tl (encode' e) @ \<C>'"
   using encode_def by (induction e arbitrary: \<C>') fastforce+
 
 lemma encode_to_apply [dest]: "encode' e @ \<C>' = Apply\<^sub>e # \<C> \<Longrightarrow> False"
@@ -255,8 +257,8 @@ lemma encode_to_return [dest]: "encode' e @ \<C>' = Return\<^sub>e # \<C> \<Long
 lemma encode_to_jump [dest]: "encode' e @ \<C>' = Jump\<^sub>e # \<C> \<Longrightarrow> False"
   by (induction e arbitrary: \<C>') simp_all
 
-lemma encode_lam_closure [dest]: "Lam\<^sub>e env \<C> = encode_closure c \<Longrightarrow> 
-    \<exists>t \<Delta> e. c = Lam\<^sub>c t \<Delta> e \<and> env = map encode_closure \<Delta> \<and> \<C> = encode e"
+lemma encode_lam_closure [dest]: "Lam\<^sub>e env \<C> n = encode_closure c \<Longrightarrow> 
+    \<exists>t \<Delta> e. c = Fun\<^sub>g t \<Delta> e n \<and> env = map (map encode_closure) \<Delta> \<and> \<C> = encode e"
   by (induction c) simp_all
 
 lemma prepend_frame_to_cons [dest]: "prepend_to_top_frame \<C>' s\<^sub>e = (\<Delta>, \<C>) # s\<^sub>e' \<Longrightarrow> 
@@ -264,7 +266,7 @@ lemma prepend_frame_to_cons [dest]: "prepend_to_top_frame \<C>' s\<^sub>e = (\<D
   by (induction \<C>' s\<^sub>e rule: prepend_to_top_frame.induct) simp_all
 
 lemma prepend_env_to_cons [dest]: "prepend_to_top_env c s\<^sub>e = (\<Delta>, \<C>) # s\<^sub>e' \<Longrightarrow> 
-    \<exists>\<Delta>'. s\<^sub>e = (\<Delta>', \<C>) # s\<^sub>e' \<and> \<Delta> = c # \<Delta>'"
+    \<exists>\<Delta>'. s\<^sub>e = (\<Delta>', \<C>) # s\<^sub>e' \<and> \<Delta> = cons_fst c \<Delta>'"
   by (induction c s\<^sub>e rule: prepend_to_top_env.induct) simp_all
 
 lemma prepend_to_apply [dest]: "prepend_to_top_frame (encode' e) s\<^sub>e = (\<Delta>, Apply\<^sub>e # \<C>) # s\<^sub>e' \<Longrightarrow> 
@@ -287,255 +289,258 @@ lemma prepend_to_jump [dest]: "prepend_to_top_frame (encode' e) s\<^sub>e = (\<D
     False"
   by (induction "encode' e" s\<^sub>e rule: prepend_to_top_frame.induct) auto
 
-lemma encode_stack_to_lookup [dest]: "stack_from_stack s\<^sub>c = (\<Delta>\<^sub>e, Lookup\<^sub>e x y z # \<C>) # s\<^sub>e \<Longrightarrow> 
-  \<exists>\<Delta>\<^sub>c e s\<^sub>c' \<C>'. s\<^sub>c = FApp1\<^sub>c \<Delta>\<^sub>c e # s\<^sub>c' \<and> stack_from_stack s\<^sub>c' = (\<Delta>\<^sub>e, \<C>') # s\<^sub>e \<and> 
-    head_expr e = Var\<^sub>d x \<and> \<C> = tl (encode' e) @ Apply\<^sub>e # \<C>' \<and> y = 0 \<and> z = 0"
-proof (induction s\<^sub>c rule: stack_from_stack.induct)
-  case (2 \<Delta> e s\<^sub>c)
-  then obtain \<C>' where "stack_from_stack s\<^sub>c = (\<Delta>\<^sub>e, \<C>') # s\<^sub>e \<and> 
-    encode' e @ Apply\<^sub>e # \<C>' = Lookup\<^sub>e x y z # \<C>" by fastforce
+lemma encode_stack_to_lookup [dest]: "stack_from_stack s\<^sub>g = (\<Delta>\<^sub>e, Lookup\<^sub>e x y # \<C>) # s\<^sub>e \<Longrightarrow> 
+  \<exists>\<Delta>\<^sub>g e s\<^sub>g' \<C>'. s\<^sub>g = FApp1\<^sub>g \<Delta>\<^sub>g e # s\<^sub>g' \<and> stack_from_stack s\<^sub>g' = (\<Delta>\<^sub>e, \<C>') # s\<^sub>e \<and> 
+    head_expr e = Var\<^sub>g x y \<and> \<C> = tl (encode' e) @ Apply\<^sub>e # \<C>'"
+proof (induction s\<^sub>g rule: stack_from_stack.induct)
+  case (2 \<Delta> e s\<^sub>g)
+  then obtain \<C>' where "stack_from_stack s\<^sub>g = (\<Delta>\<^sub>e, \<C>') # s\<^sub>e \<and> 
+    encode' e @ Apply\<^sub>e # \<C>' = Lookup\<^sub>e x y # \<C>" by fastforce
   thus ?case by auto
 qed auto
 
-lemma encode_stack_to_pushcon [dest]: "stack_from_stack s\<^sub>c = (\<Delta>\<^sub>e, PushCon\<^sub>e n # \<C>) # s\<^sub>e \<Longrightarrow> 
-  \<exists>\<Delta>\<^sub>c e s\<^sub>c' \<C>'. s\<^sub>c = FApp1\<^sub>c \<Delta>\<^sub>c e # s\<^sub>c' \<and> stack_from_stack s\<^sub>c' = (\<Delta>\<^sub>e, \<C>') # s\<^sub>e \<and> 
-    head_expr e = Const\<^sub>d n \<and> \<C> = tl (encode' e) @ Apply\<^sub>e # \<C>'"
-proof (induction s\<^sub>c rule: stack_from_stack.induct)
-  case (2 \<Delta>\<^sub>s e s\<^sub>c)
-  then obtain \<C>' where "stack_from_stack s\<^sub>c = (\<Delta>\<^sub>e, \<C>') # s\<^sub>e \<and> 
+lemma encode_stack_to_pushcon [dest]: "stack_from_stack s\<^sub>g = (\<Delta>\<^sub>e, PushCon\<^sub>e n # \<C>) # s\<^sub>e \<Longrightarrow> 
+  \<exists>\<Delta>\<^sub>g e s\<^sub>g' \<C>'. s\<^sub>g = FApp1\<^sub>g \<Delta>\<^sub>g e # s\<^sub>g' \<and> stack_from_stack s\<^sub>g' = (\<Delta>\<^sub>e, \<C>') # s\<^sub>e \<and> 
+    head_expr e = Const\<^sub>g n \<and> \<C> = tl (encode' e) @ Apply\<^sub>e # \<C>'"
+proof (induction s\<^sub>g rule: stack_from_stack.induct)
+  case (2 \<Delta>\<^sub>s e s\<^sub>g)
+  then obtain \<C>' where "stack_from_stack s\<^sub>g = (\<Delta>\<^sub>e, \<C>') # s\<^sub>e \<and> 
     encode' e @ Apply\<^sub>e # \<C>' = PushCon\<^sub>e n # \<C>" by fastforce
   thus ?case by auto
 qed auto
 
-lemma encode_stack_to_pushlam [dest]: "stack_from_stack s\<^sub>c = (\<Delta>\<^sub>e, PushLam\<^sub>e \<C>' n # \<C>) # s\<^sub>e \<Longrightarrow> 
-  \<exists>\<Delta>\<^sub>c e s\<^sub>c' t e' \<C>''. s\<^sub>c = FApp1\<^sub>c \<Delta>\<^sub>c e # s\<^sub>c' \<and> stack_from_stack s\<^sub>c' = (\<Delta>\<^sub>e, \<C>'') # s\<^sub>e \<and> 
-    head_expr e = Lam\<^sub>d t e' \<and> \<C> = tl (encode' e) @ Apply\<^sub>e # \<C>'' \<and> \<C>' = encode e' \<and> 
-      n = length (strip_lets e')"
-proof (induction s\<^sub>c rule: stack_from_stack.induct)
-  case (2 \<Delta>\<^sub>c e s\<^sub>c)
-  then obtain \<C>'' where "stack_from_stack s\<^sub>c = (\<Delta>\<^sub>e, \<C>'') # s\<^sub>e \<and> 
+lemma encode_stack_to_pushlam [dest]: "stack_from_stack s\<^sub>g = (\<Delta>\<^sub>e, PushLam\<^sub>e \<C>' n # \<C>) # s\<^sub>e \<Longrightarrow> 
+  \<exists>\<Delta>\<^sub>g e s\<^sub>g' t e' \<C>''. s\<^sub>g = FApp1\<^sub>g \<Delta>\<^sub>g e # s\<^sub>g' \<and> stack_from_stack s\<^sub>g' = (\<Delta>\<^sub>e, \<C>'') # s\<^sub>e \<and> 
+    head_expr e = Lam\<^sub>g t e' n \<and> \<C> = tl (encode' e) @ Apply\<^sub>e # \<C>'' \<and> \<C>' = encode e'"
+proof (induction s\<^sub>g rule: stack_from_stack.induct)
+  case (2 \<Delta>\<^sub>g e s\<^sub>g)
+  then obtain \<C>'' where "stack_from_stack s\<^sub>g = (\<Delta>\<^sub>e, \<C>'') # s\<^sub>e \<and> 
     encode' e @ Apply\<^sub>e # \<C>'' = PushLam\<^sub>e \<C>' n # \<C>" by fastforce
-  moreover then obtain t e' where "head_expr e = Lam\<^sub>d t e' \<and> \<C>' = encode e' \<and> 
-    \<C> = tl (encode' e) @ Apply\<^sub>e # \<C>'' \<and> n = length (strip_lets e')" by (metis encode_to_pushlam)
+  moreover then obtain t e' where "head_expr e = Lam\<^sub>g t e' n \<and> \<C>' = encode e' \<and> 
+    \<C> = tl (encode' e) @ Apply\<^sub>e # \<C>''" by (metis encode_to_pushlam)
   ultimately show ?case by auto
 qed auto
 
 lemma encode_stack_to_apply [dest]: "stack_from_stack s = (\<Delta>\<^sub>e, Apply\<^sub>e # \<C>) # s\<^sub>e \<Longrightarrow> 
-    \<exists>s\<^sub>c' c. s = FApp2\<^sub>c c # s\<^sub>c' \<and> stack_from_stack s\<^sub>c' = (\<Delta>\<^sub>e, \<C>) # s\<^sub>e"
+    \<exists>s\<^sub>g' c. s = FApp2\<^sub>g c # s\<^sub>g' \<and> stack_from_stack s\<^sub>g' = (\<Delta>\<^sub>e, \<C>) # s\<^sub>e"
   by (induction s rule: stack_from_stack.induct) auto
 
 lemma encode_stack_to_pushenv [dest]: "stack_from_stack s = (\<Delta>\<^sub>e, PushEnv\<^sub>e # \<C>) # s\<^sub>e \<Longrightarrow> 
-  \<exists>s\<^sub>c' \<Delta> e \<C>'. s = FLet\<^sub>c \<Delta> e # s\<^sub>c' \<and> \<C> = encode' e @ PopEnv\<^sub>e # \<C>' \<and> 
-    stack_from_stack s\<^sub>c' = (\<Delta>\<^sub>e, \<C>') # s\<^sub>e"
+  \<exists>s\<^sub>g' \<Delta> e \<C>'. s = FLet\<^sub>g \<Delta> e # s\<^sub>g' \<and> \<C> = encode' e @ PopEnv\<^sub>e # \<C>' \<and> 
+    stack_from_stack s\<^sub>g' = (\<Delta>\<^sub>e, \<C>') # s\<^sub>e"
   by (induction s rule: stack_from_stack.induct) auto
 
 lemma encode_stack_to_popenv [dest]: "stack_from_stack s = (\<Delta>\<^sub>e, PopEnv\<^sub>e # \<C>) # s\<^sub>e \<Longrightarrow> 
-  \<exists>s\<^sub>c' c \<Delta>\<^sub>e'. s = FPop\<^sub>c c # s\<^sub>c' \<and> \<Delta>\<^sub>e = encode_closure c # \<Delta>\<^sub>e' \<and> 
-    stack_from_stack s\<^sub>c' = (\<Delta>\<^sub>e', \<C>) # s\<^sub>e"
+  \<exists>s\<^sub>g' c \<Delta>\<^sub>e'. s = FPop\<^sub>g c # s\<^sub>g' \<and> \<Delta>\<^sub>e = cons_fst (encode_closure c) \<Delta>\<^sub>e' \<and> 
+    stack_from_stack s\<^sub>g' = (\<Delta>\<^sub>e', \<C>) # s\<^sub>e"
 proof (induction s rule: stack_from_stack.induct)
-  case (5 c s\<^sub>c)
-  hence "prepend_to_top_env (encode_closure c) (stack_from_stack s\<^sub>c) = (\<Delta>\<^sub>e, \<C>) # s\<^sub>e" by auto
-  then obtain \<Delta>' where "stack_from_stack s\<^sub>c = (\<Delta>', \<C>) # s\<^sub>e \<and> \<Delta>\<^sub>e = encode_closure c # \<Delta>'" by auto
+  case (5 c s\<^sub>g)
+  hence "prepend_to_top_env (encode_closure c) (stack_from_stack s\<^sub>g) = (\<Delta>\<^sub>e, \<C>) # s\<^sub>e" by auto
+  then obtain \<Delta>' where "stack_from_stack s\<^sub>g = (\<Delta>', \<C>) # s\<^sub>e \<and> \<Delta>\<^sub>e = cons_fst (encode_closure c) \<Delta>'" 
+    by auto
   then show ?case by auto
 qed auto
 
 lemma encode_stack_to_return [dest]: "stack_from_stack s = (\<Delta>\<^sub>e, Return\<^sub>e # \<C>) # s\<^sub>e \<Longrightarrow> 
-  \<exists>\<Delta>\<^sub>c s\<^sub>c'. s = FReturn\<^sub>c \<Delta>\<^sub>c # s\<^sub>c' \<and> \<Delta>\<^sub>e = map encode_closure \<Delta>\<^sub>c \<and> s\<^sub>e = stack_from_stack s\<^sub>c' \<and> 
+  \<exists>\<Delta>\<^sub>g s\<^sub>g'. s = FReturn\<^sub>g \<Delta>\<^sub>g # s\<^sub>g' \<and> \<Delta>\<^sub>e = map (map encode_closure) \<Delta>\<^sub>g \<and> s\<^sub>e = stack_from_stack s\<^sub>g' \<and> 
     \<C> = []"
   by (induction s rule: stack_from_stack.induct) auto
 
 lemma encode_stack_to_jump [dest]: "stack_from_stack s = (\<Delta>\<^sub>e, Jump\<^sub>e # \<C>) # s\<^sub>e \<Longrightarrow> False"
   by (induction s rule: stack_from_stack.induct) auto
 
-lemma encode_state_to_lookup [dest, consumes 1, case_names SE\<^sub>c SC\<^sub>c]: "
-  encode_state \<Sigma>\<^sub>c = S\<^sub>e \<V> ((\<Delta>\<^sub>e, Lookup\<^sub>e x y z # \<C>) # s\<^sub>e) \<Longrightarrow> 
-    (\<And>s\<^sub>c \<Delta>\<^sub>c e \<C>'. head_expr e = Var\<^sub>d x \<Longrightarrow> y = 0 \<Longrightarrow> z = 0 \<Longrightarrow> \<C> = tl (encode' e) @ \<C>' \<Longrightarrow> 
-      stack_from_stack s\<^sub>c = ((\<Delta>\<^sub>e, \<C>') # s\<^sub>e) \<Longrightarrow> \<V> = vals_from_stack s\<^sub>c \<Longrightarrow> P (SE\<^sub>c s\<^sub>c \<Delta>\<^sub>c e)) \<Longrightarrow> 
-    (\<And>s\<^sub>c c \<Delta>\<^sub>c e \<C>'. head_expr e = Var\<^sub>d x \<Longrightarrow> y = 0 \<Longrightarrow> z = 0 \<Longrightarrow> 
-      \<C> = tl (encode' e) @ Apply\<^sub>e # \<C>' \<Longrightarrow> stack_from_stack s\<^sub>c = ((\<Delta>\<^sub>e, \<C>') # s\<^sub>e) \<Longrightarrow> 
-      \<V> = encode_closure c # vals_from_stack s\<^sub>c \<Longrightarrow> P (SC\<^sub>c (FApp1\<^sub>c \<Delta>\<^sub>c e # s\<^sub>c) c)) \<Longrightarrow> P \<Sigma>\<^sub>c"
-proof (induction \<Sigma>\<^sub>c)
-  case (SE\<^sub>c s \<Delta> e)
+lemma encode_state_to_lookup [dest, consumes 1, case_names SE\<^sub>g SC\<^sub>g]: "
+  encode_state \<Sigma>\<^sub>g = S\<^sub>e \<V> ((\<Delta>\<^sub>e, Lookup\<^sub>e x y # \<C>) # s\<^sub>e) \<Longrightarrow> 
+    (\<And>s\<^sub>g \<Delta>\<^sub>g e \<C>'. head_expr e = Var\<^sub>g x y \<Longrightarrow> \<C> = tl (encode' e) @ \<C>' \<Longrightarrow> 
+      stack_from_stack s\<^sub>g = ((\<Delta>\<^sub>e, \<C>') # s\<^sub>e) \<Longrightarrow> \<V> = vals_from_stack s\<^sub>g \<Longrightarrow> P (SE\<^sub>g s\<^sub>g \<Delta>\<^sub>g e)) \<Longrightarrow> 
+    (\<And>s\<^sub>g c \<Delta>\<^sub>g e \<C>'. head_expr e = Var\<^sub>g x y \<Longrightarrow> 
+      \<C> = tl (encode' e) @ Apply\<^sub>e # \<C>' \<Longrightarrow> stack_from_stack s\<^sub>g = ((\<Delta>\<^sub>e, \<C>') # s\<^sub>e) \<Longrightarrow> 
+      \<V> = encode_closure c # vals_from_stack s\<^sub>g \<Longrightarrow> P (SC\<^sub>g (FApp1\<^sub>g \<Delta>\<^sub>g e # s\<^sub>g) c)) \<Longrightarrow> P \<Sigma>\<^sub>g"
+proof (induction \<Sigma>\<^sub>g)
+  case (SE\<^sub>g s \<Delta> e)
   moreover then obtain \<C>' where "stack_from_stack s = (\<Delta>\<^sub>e, \<C>') # s\<^sub>e \<and> 
-    encode' e @ \<C>' = Lookup\<^sub>e x y z # \<C>" by auto
+    encode' e @ \<C>' = Lookup\<^sub>e x y # \<C>" by auto
   ultimately show ?case by auto
 qed auto
 
-lemma encode_state_to_pushcon [dest, consumes 1, case_names SE\<^sub>c SC\<^sub>c]: "
-  encode_state \<Sigma>\<^sub>c = S\<^sub>e \<V> ((\<Delta>\<^sub>e, PushCon\<^sub>e n # \<C>) # s\<^sub>e) \<Longrightarrow> 
-    (\<And>s\<^sub>c \<Delta>\<^sub>c e \<C>'. head_expr e = Const\<^sub>d n \<Longrightarrow> \<C> = tl (encode' e) @ \<C>' \<Longrightarrow> 
-      stack_from_stack s\<^sub>c = ((\<Delta>\<^sub>e, \<C>') # s\<^sub>e) \<Longrightarrow> \<V> = vals_from_stack s\<^sub>c \<Longrightarrow> P (SE\<^sub>c s\<^sub>c \<Delta>\<^sub>c e)) \<Longrightarrow> 
-    (\<And>s\<^sub>c c \<Delta>\<^sub>c e \<C>'. head_expr e = Const\<^sub>d n \<Longrightarrow> \<C> = tl (encode' e) @ Apply\<^sub>e # \<C>' \<Longrightarrow> 
-      stack_from_stack s\<^sub>c = ((\<Delta>\<^sub>e, \<C>') # s\<^sub>e) \<Longrightarrow> \<V> = encode_closure c # vals_from_stack s\<^sub>c \<Longrightarrow> 
-      P (SC\<^sub>c (FApp1\<^sub>c \<Delta>\<^sub>c e # s\<^sub>c) c)) \<Longrightarrow> P \<Sigma>\<^sub>c"
-proof (induction \<Sigma>\<^sub>c)
-  case (SE\<^sub>c s \<Delta> e)
+lemma encode_state_to_pushcon [dest, consumes 1, case_names SE\<^sub>g SC\<^sub>g]: "
+  encode_state \<Sigma>\<^sub>g = S\<^sub>e \<V> ((\<Delta>\<^sub>e, PushCon\<^sub>e n # \<C>) # s\<^sub>e) \<Longrightarrow> 
+    (\<And>s\<^sub>g \<Delta>\<^sub>g e \<C>'. head_expr e = Const\<^sub>g n \<Longrightarrow> \<C> = tl (encode' e) @ \<C>' \<Longrightarrow> 
+      stack_from_stack s\<^sub>g = ((\<Delta>\<^sub>e, \<C>') # s\<^sub>e) \<Longrightarrow> \<V> = vals_from_stack s\<^sub>g \<Longrightarrow> P (SE\<^sub>g s\<^sub>g \<Delta>\<^sub>g e)) \<Longrightarrow> 
+    (\<And>s\<^sub>g c \<Delta>\<^sub>g e \<C>'. head_expr e = Const\<^sub>g n \<Longrightarrow> \<C> = tl (encode' e) @ Apply\<^sub>e # \<C>' \<Longrightarrow> 
+      stack_from_stack s\<^sub>g = ((\<Delta>\<^sub>e, \<C>') # s\<^sub>e) \<Longrightarrow> \<V> = encode_closure c # vals_from_stack s\<^sub>g \<Longrightarrow> 
+      P (SC\<^sub>g (FApp1\<^sub>g \<Delta>\<^sub>g e # s\<^sub>g) c)) \<Longrightarrow> P \<Sigma>\<^sub>g"
+proof (induction \<Sigma>\<^sub>g)
+  case (SE\<^sub>g s \<Delta> e)
   moreover then obtain \<C>' where "stack_from_stack s = (\<Delta>\<^sub>e, \<C>') # s\<^sub>e \<and> 
     encode' e @ \<C>' = PushCon\<^sub>e n # \<C>" by auto
   ultimately show ?case by auto
 qed auto
 
-lemma encode_state_to_pushlam [dest, consumes 1, case_names SE\<^sub>c SC\<^sub>c]: "
-  encode_state \<Sigma>\<^sub>c = S\<^sub>e \<V> ((\<Delta>\<^sub>e, PushLam\<^sub>e \<C>' n # \<C>) # s\<^sub>e) \<Longrightarrow> 
-    (\<And>s\<^sub>c \<Delta>\<^sub>c e tt e' \<C>''. \<Sigma>\<^sub>c = SE\<^sub>c s\<^sub>c \<Delta>\<^sub>c e \<Longrightarrow> head_expr e = Lam\<^sub>d tt e' \<Longrightarrow> 
-      \<C> = tl (encode' e) @ \<C>'' \<Longrightarrow> \<C>' = encode e' \<Longrightarrow> n = length (strip_lets e') \<Longrightarrow> 
-      \<V> = vals_from_stack s\<^sub>c \<Longrightarrow> stack_from_stack s\<^sub>c = (\<Delta>\<^sub>e, \<C>'') # s\<^sub>e \<Longrightarrow> P) \<Longrightarrow> 
-    (\<And>s\<^sub>c c \<Delta>\<^sub>c e tt e' \<C>''. \<Sigma>\<^sub>c = SC\<^sub>c (FApp1\<^sub>c \<Delta>\<^sub>c e # s\<^sub>c) c \<Longrightarrow> head_expr e = Lam\<^sub>d tt e' \<Longrightarrow> 
-      \<C> = tl (encode' e) @ Apply\<^sub>e # \<C>'' \<Longrightarrow> \<C>' = encode e' \<Longrightarrow> n = length (strip_lets e') \<Longrightarrow> 
-      \<V> = encode_closure c # vals_from_stack s\<^sub>c \<Longrightarrow> stack_from_stack s\<^sub>c = (\<Delta>\<^sub>e, \<C>'') # s\<^sub>e \<Longrightarrow> P) \<Longrightarrow> 
+lemma encode_state_to_pushlam [dest, consumes 1, case_names SE\<^sub>g SC\<^sub>g]: "
+  encode_state \<Sigma>\<^sub>g = S\<^sub>e \<V> ((\<Delta>\<^sub>e, PushLam\<^sub>e \<C>' n # \<C>) # s\<^sub>e) \<Longrightarrow> 
+    (\<And>s\<^sub>g \<Delta>\<^sub>g e tt e' \<C>''. \<Sigma>\<^sub>g = SE\<^sub>g s\<^sub>g \<Delta>\<^sub>g e \<Longrightarrow> head_expr e = Lam\<^sub>g tt e' n \<Longrightarrow> 
+      \<C> = tl (encode' e) @ \<C>'' \<Longrightarrow> \<C>' = encode e' \<Longrightarrow> 
+      \<V> = vals_from_stack s\<^sub>g \<Longrightarrow> stack_from_stack s\<^sub>g = (\<Delta>\<^sub>e, \<C>'') # s\<^sub>e \<Longrightarrow> P) \<Longrightarrow> 
+    (\<And>s\<^sub>g c \<Delta>\<^sub>g e tt e' \<C>''. \<Sigma>\<^sub>g = SC\<^sub>g (FApp1\<^sub>g \<Delta>\<^sub>g e # s\<^sub>g) c \<Longrightarrow> head_expr e = Lam\<^sub>g tt e' n \<Longrightarrow> 
+      \<C> = tl (encode' e) @ Apply\<^sub>e # \<C>'' \<Longrightarrow> \<C>' = encode e' \<Longrightarrow> 
+      \<V> = encode_closure c # vals_from_stack s\<^sub>g \<Longrightarrow> stack_from_stack s\<^sub>g = (\<Delta>\<^sub>e, \<C>'') # s\<^sub>e \<Longrightarrow> P) \<Longrightarrow> 
     P"
-proof (induction \<Sigma>\<^sub>c)
-  case (SE\<^sub>c s\<^sub>c \<Delta>\<^sub>c e)
-  moreover then obtain \<C>'' where "stack_from_stack s\<^sub>c = (\<Delta>\<^sub>e, \<C>'') # s\<^sub>e \<and> 
+proof (induction \<Sigma>\<^sub>g)
+  case (SE\<^sub>g s\<^sub>g \<Delta>\<^sub>g e)
+  moreover then obtain \<C>'' where "stack_from_stack s\<^sub>g = (\<Delta>\<^sub>e, \<C>'') # s\<^sub>e \<and> 
     encode' e @ \<C>'' = PushLam\<^sub>e \<C>' n # \<C>" by auto
-  moreover then obtain tt e' where "head_expr e = Lam\<^sub>d tt e' \<and> \<C>' = encode e' \<and> 
-    \<C> = tl (encode' e) @ \<C>'' \<and> n = length (strip_lets e')" by (metis encode_to_pushlam)
+  moreover then obtain tt e' where "head_expr e = Lam\<^sub>g tt e' n \<and> \<C>' = encode e' \<and> 
+    \<C> = tl (encode' e) @ \<C>''" by (metis encode_to_pushlam)
   ultimately show ?case by auto
 qed auto
 
 lemma encode_state_to_apply [dest]: "
-  encode_state \<Sigma>\<^sub>c = S\<^sub>e (v # Lam\<^sub>e \<Delta>\<^sub>e' \<C>' # \<V>) ((\<Delta>\<^sub>e, Apply\<^sub>e # \<C>) # s\<^sub>e) \<Longrightarrow>
-    \<exists>s\<^sub>c c c'. \<Sigma>\<^sub>c = SC\<^sub>c (FApp2\<^sub>c c' # s\<^sub>c) c \<and> stack_from_stack s\<^sub>c = ((\<Delta>\<^sub>e, \<C>) # s\<^sub>e) \<and> 
-      v = encode_closure c \<and> Lam\<^sub>e \<Delta>\<^sub>e' \<C>' = encode_closure c' \<and> \<V> = vals_from_stack s\<^sub>c"
-  by (induction \<Sigma>\<^sub>c) auto
+  encode_state \<Sigma>\<^sub>g = S\<^sub>e (v # Lam\<^sub>e \<Delta>\<^sub>e' \<C>' n # \<V>) ((\<Delta>\<^sub>e, Apply\<^sub>e # \<C>) # s\<^sub>e) \<Longrightarrow>
+    \<exists>s\<^sub>g c c'. \<Sigma>\<^sub>g = SC\<^sub>g (FApp2\<^sub>g c' # s\<^sub>g) c \<and> stack_from_stack s\<^sub>g = ((\<Delta>\<^sub>e, \<C>) # s\<^sub>e) \<and> 
+      v = encode_closure c \<and> Lam\<^sub>e \<Delta>\<^sub>e' \<C>' n = encode_closure c' \<and> \<V> = vals_from_stack s\<^sub>g"
+  by (induction \<Sigma>\<^sub>g) auto
 
-lemma encode_state_to_pushenv [dest]: "encode_state \<Sigma>\<^sub>c = S\<^sub>e (v # \<V>) ((\<Delta>\<^sub>e, PushEnv\<^sub>e # \<C>) # s\<^sub>e) \<Longrightarrow> 
-  \<exists>c s\<^sub>c. \<Sigma>\<^sub>c = SC\<^sub>c s\<^sub>c c \<and> v = encode_closure c \<and> \<V> = vals_from_stack s\<^sub>c \<and> 
-    stack_from_stack s\<^sub>c = (\<Delta>\<^sub>e, PushEnv\<^sub>e # \<C>) # s\<^sub>e"
-  by (induction \<Sigma>\<^sub>c) auto
+lemma encode_state_to_pushenv [dest]: "encode_state \<Sigma>\<^sub>g = S\<^sub>e (v # \<V>) ((\<Delta>\<^sub>e, PushEnv\<^sub>e # \<C>) # s\<^sub>e) \<Longrightarrow> 
+  \<exists>c s\<^sub>g. \<Sigma>\<^sub>g = SC\<^sub>g s\<^sub>g c \<and> v = encode_closure c \<and> \<V> = vals_from_stack s\<^sub>g \<and> 
+    stack_from_stack s\<^sub>g = (\<Delta>\<^sub>e, PushEnv\<^sub>e # \<C>) # s\<^sub>e"
+  by (induction \<Sigma>\<^sub>g) auto
 
-lemma encode_state_to_popenv [dest]: "encode_state \<Sigma>\<^sub>c = S\<^sub>e \<V> ((v # \<Delta>\<^sub>e, PopEnv\<^sub>e # \<C>) # s\<^sub>e) \<Longrightarrow>
-  \<exists>c s\<^sub>c. \<Sigma>\<^sub>c = SC\<^sub>c s\<^sub>c c \<and> \<V> = encode_closure c # vals_from_stack s\<^sub>c \<and> 
-    stack_from_stack s\<^sub>c = (v # \<Delta>\<^sub>e, PopEnv\<^sub>e # \<C>) # s\<^sub>e"
-  by (induction \<Sigma>\<^sub>c) auto
+lemma encode_state_to_popenv [dest]: "encode_state \<Sigma>\<^sub>g = S\<^sub>e \<V> ((cons_fst v \<Delta>\<^sub>e, PopEnv\<^sub>e # \<C>) # s\<^sub>e) \<Longrightarrow>
+  \<exists>c s\<^sub>g. \<Sigma>\<^sub>g = SC\<^sub>g s\<^sub>g c \<and> \<V> = encode_closure c # vals_from_stack s\<^sub>g \<and> 
+    stack_from_stack s\<^sub>g = (cons_fst v \<Delta>\<^sub>e, PopEnv\<^sub>e # \<C>) # s\<^sub>e"
+  by (induction \<Sigma>\<^sub>g) auto
 
-lemma encode_state_to_return [dest]: "encode_state \<Sigma>\<^sub>c = S\<^sub>e \<V> ((\<Delta>\<^sub>e, Return\<^sub>e # \<C>) # s\<^sub>e) \<Longrightarrow> 
-  \<exists>\<Delta>\<^sub>c s c. \<Sigma>\<^sub>c = SC\<^sub>c (FReturn\<^sub>c \<Delta>\<^sub>c # s) c \<and> s\<^sub>e = stack_from_stack s \<and>
-    \<Delta>\<^sub>e = map encode_closure \<Delta>\<^sub>c \<and> \<V> = encode_closure c # vals_from_stack s \<and> \<C> = []"
-  by (induction \<Sigma>\<^sub>c) auto
+lemma encode_state_to_return [dest]: "encode_state \<Sigma>\<^sub>g = S\<^sub>e \<V> ((\<Delta>\<^sub>e, Return\<^sub>e # \<C>) # s\<^sub>e) \<Longrightarrow> 
+  \<exists>\<Delta>\<^sub>g s c. \<Sigma>\<^sub>g = SC\<^sub>g (FReturn\<^sub>g \<Delta>\<^sub>g # s) c \<and> s\<^sub>e = stack_from_stack s \<and>
+    \<Delta>\<^sub>e = map (map encode_closure) \<Delta>\<^sub>g \<and> \<V> = encode_closure c # vals_from_stack s \<and> \<C> = []"
+  by (induction \<Sigma>\<^sub>g) auto
 
-lemma encode_state_to_jump [dest]: "encode_state \<Sigma>\<^sub>c = S\<^sub>e \<V> ((\<Delta>\<^sub>e, Jump\<^sub>e # \<C>) # s\<^sub>e) \<Longrightarrow> False"
-  by (induction \<Sigma>\<^sub>c) auto
+lemma encode_state_to_jump [dest]: "encode_state \<Sigma>\<^sub>g = S\<^sub>e \<V> ((\<Delta>\<^sub>e, Jump\<^sub>e # \<C>) # s\<^sub>e) \<Longrightarrow> False"
+  by (induction \<Sigma>\<^sub>g) auto
 
 text \<open>And now, we can finally prove completeness.\<close>
 
-theorem complete\<^sub>e [simp]: "encode_state \<Sigma>\<^sub>c \<leadsto>\<^sub>e \<Sigma>\<^sub>t' \<Longrightarrow> \<Sigma>\<^sub>c :\<^sub>c t \<Longrightarrow>
-  \<exists>\<Sigma>\<^sub>c'. iter (\<leadsto>\<^sub>c) \<Sigma>\<^sub>c \<Sigma>\<^sub>c' \<and> \<Sigma>\<^sub>t' = encode_state \<Sigma>\<^sub>c'"
-proof (induction "encode_state \<Sigma>\<^sub>c" \<Sigma>\<^sub>t' rule: eval\<^sub>e.induct)
-  case (ev\<^sub>e_lookup \<Delta>\<^sub>e x v \<V> y z \<C> s\<^sub>e)
-  hence X: "encode_state \<Sigma>\<^sub>c = S\<^sub>e \<V> ((\<Delta>\<^sub>e, Lookup\<^sub>e x y z # \<C>) # s\<^sub>e)" by simp
+theorem complete\<^sub>e [simp]: "encode_state \<Sigma>\<^sub>g \<leadsto>\<^sub>e \<Sigma>\<^sub>t' \<Longrightarrow> \<Sigma>\<^sub>g :\<^sub>g t \<Longrightarrow>
+  \<exists>\<Sigma>\<^sub>g'. iter (\<leadsto>\<^sub>g) \<Sigma>\<^sub>g \<Sigma>\<^sub>g' \<and> \<Sigma>\<^sub>t' = encode_state \<Sigma>\<^sub>g'"
+proof (induction "encode_state \<Sigma>\<^sub>g" \<Sigma>\<^sub>t' rule: eval\<^sub>e.induct)
+  case (ev\<^sub>e_lookup \<Delta>\<^sub>e x vs y v \<V> \<C> s\<^sub>e)
+  hence X: "encode_state \<Sigma>\<^sub>g = S\<^sub>e \<V> ((\<Delta>\<^sub>e, Lookup\<^sub>e x y # \<C>) # s\<^sub>e)" by simp
   from X ev\<^sub>e_lookup(1, 3) show ?case
   proof (induction rule: encode_state_to_lookup)
-    case (SE\<^sub>c s\<^sub>c \<Delta>\<^sub>c e \<C>')
-    have X: "iter (\<leadsto>\<^sub>c) (SE\<^sub>c s\<^sub>c \<Delta>\<^sub>c e) (SE\<^sub>c (tail_expr \<Delta>\<^sub>c e @ s\<^sub>c) \<Delta>\<^sub>c (head_expr e))" by simp
-    from SE\<^sub>c obtain c where C: "lookup \<Delta>\<^sub>c x = Some c \<and> encode_closure c = v" by fastforce
-    with X SE\<^sub>c have "iter (\<leadsto>\<^sub>c) (SE\<^sub>c s\<^sub>c \<Delta>\<^sub>c e) (SC\<^sub>c (tail_expr \<Delta>\<^sub>c e @ s\<^sub>c) c)" by simp
-    with SE\<^sub>c C show ?case by auto
+    case (SE\<^sub>g s\<^sub>g \<Delta>\<^sub>g e \<C>')
+    have X: "iter (\<leadsto>\<^sub>g) (SE\<^sub>g s\<^sub>g \<Delta>\<^sub>g e) (SE\<^sub>g (tail_expr \<Delta>\<^sub>g e @ s\<^sub>g) \<Delta>\<^sub>g (head_expr e))" by simp
+    from SE\<^sub>g obtain cs c where C: "lookup \<Delta>\<^sub>g x = Some cs \<and> lookup cs y = Some c \<and> 
+      encode_closure c = v" by fastforce
+    with X SE\<^sub>g have "iter (\<leadsto>\<^sub>g) (SE\<^sub>g s\<^sub>g \<Delta>\<^sub>g e) (SC\<^sub>g (tail_expr \<Delta>\<^sub>g e @ s\<^sub>g) c)" by simp
+    with SE\<^sub>g C show ?case by auto
   next
-    case (SC\<^sub>c s\<^sub>c c \<Delta>\<^sub>c e \<C>')
-    moreover have "iter (\<leadsto>\<^sub>c) (SE\<^sub>c (FApp2\<^sub>c c # s\<^sub>c) \<Delta>\<^sub>c e) 
-      (SE\<^sub>c (tail_expr \<Delta>\<^sub>c e @ FApp2\<^sub>c c # s\<^sub>c) \<Delta>\<^sub>c (head_expr e))" by simp
-    moreover have "SC\<^sub>c (FApp1\<^sub>c \<Delta>\<^sub>c e # s\<^sub>c) c \<leadsto>\<^sub>c SE\<^sub>c (FApp2\<^sub>c c # s\<^sub>c) \<Delta>\<^sub>c e" by simp
-    ultimately have X: "iter (\<leadsto>\<^sub>c) (SC\<^sub>c (FApp1\<^sub>c \<Delta>\<^sub>c e # s\<^sub>c) c) 
-      (SE\<^sub>c (tail_expr \<Delta>\<^sub>c e @ FApp2\<^sub>c c # s\<^sub>c) \<Delta>\<^sub>c (Var\<^sub>d x))" by (metis iter_step)
-    from SC\<^sub>c obtain c' where C: "lookup \<Delta>\<^sub>c x = Some c' \<and> encode_closure c' = v" by fastforce
-    with X have "iter (\<leadsto>\<^sub>c) (SC\<^sub>c (FApp1\<^sub>c \<Delta>\<^sub>c e # s\<^sub>c) c) (SC\<^sub>c (tail_expr \<Delta>\<^sub>c e @ FApp2\<^sub>c c # s\<^sub>c) c')" 
+    case (SC\<^sub>g s\<^sub>g c \<Delta>\<^sub>g e \<C>')
+    moreover have "iter (\<leadsto>\<^sub>g) (SE\<^sub>g (FApp2\<^sub>g c # s\<^sub>g) \<Delta>\<^sub>g e) 
+      (SE\<^sub>g (tail_expr \<Delta>\<^sub>g e @ FApp2\<^sub>g c # s\<^sub>g) \<Delta>\<^sub>g (head_expr e))" by simp
+    moreover have "SC\<^sub>g (FApp1\<^sub>g \<Delta>\<^sub>g e # s\<^sub>g) c \<leadsto>\<^sub>g SE\<^sub>g (FApp2\<^sub>g c # s\<^sub>g) \<Delta>\<^sub>g e" by simp
+    ultimately have X: "iter (\<leadsto>\<^sub>g) (SC\<^sub>g (FApp1\<^sub>g \<Delta>\<^sub>g e # s\<^sub>g) c) 
+      (SE\<^sub>g (tail_expr \<Delta>\<^sub>g e @ FApp2\<^sub>g c # s\<^sub>g) \<Delta>\<^sub>g (Var\<^sub>g x y))" by (metis iter_step)
+    from SC\<^sub>g obtain cs c' where C: "lookup \<Delta>\<^sub>g x = Some cs \<and> lookup cs y = Some c' \<and> 
+      encode_closure c' = v" by fastforce
+    with X have "iter (\<leadsto>\<^sub>g) (SC\<^sub>g (FApp1\<^sub>g \<Delta>\<^sub>g e # s\<^sub>g) c) (SC\<^sub>g (tail_expr \<Delta>\<^sub>g e @ FApp2\<^sub>g c # s\<^sub>g) c')" 
       by simp
-    with SC\<^sub>c C show ?case by auto
+    with SC\<^sub>g C show ?case by auto
   qed
 next
   case (ev\<^sub>e_pushcon \<V> \<Delta>\<^sub>e n \<C> s\<^sub>e)
-  hence X: "encode_state \<Sigma>\<^sub>c = S\<^sub>e \<V> ((\<Delta>\<^sub>e, PushCon\<^sub>e n # \<C>) # s\<^sub>e)" by simp
+  hence X: "encode_state \<Sigma>\<^sub>g = S\<^sub>e \<V> ((\<Delta>\<^sub>e, PushCon\<^sub>e n # \<C>) # s\<^sub>e)" by simp
   from X ev\<^sub>e_pushcon(2) show ?case
   proof (induction rule: encode_state_to_pushcon)
-    case (SE\<^sub>c s\<^sub>c \<Delta>\<^sub>c e \<C>')
-    moreover have "iter (\<leadsto>\<^sub>c) (SE\<^sub>c s\<^sub>c \<Delta>\<^sub>c e) (SE\<^sub>c (tail_expr \<Delta>\<^sub>c e @ s\<^sub>c) \<Delta>\<^sub>c (head_expr e))" by simp
-    ultimately have "iter (\<leadsto>\<^sub>c) (SE\<^sub>c s\<^sub>c \<Delta>\<^sub>c e) (SC\<^sub>c (tail_expr \<Delta>\<^sub>c e @ s\<^sub>c) (Const\<^sub>c n))" by simp
-    with SE\<^sub>c show ?case by auto
+    case (SE\<^sub>g s\<^sub>g \<Delta>\<^sub>g e \<C>')
+    moreover have "iter (\<leadsto>\<^sub>g) (SE\<^sub>g s\<^sub>g \<Delta>\<^sub>g e) (SE\<^sub>g (tail_expr \<Delta>\<^sub>g e @ s\<^sub>g) \<Delta>\<^sub>g (head_expr e))" by simp
+    ultimately have "iter (\<leadsto>\<^sub>g) (SE\<^sub>g s\<^sub>g \<Delta>\<^sub>g e) (SC\<^sub>g (tail_expr \<Delta>\<^sub>g e @ s\<^sub>g) (Num\<^sub>g n))" by simp
+    with SE\<^sub>g show ?case by auto
   next
-    case (SC\<^sub>c s\<^sub>c c \<Delta>\<^sub>c e \<C>')
-    moreover have "iter (\<leadsto>\<^sub>c) (SE\<^sub>c (FApp2\<^sub>c c # s\<^sub>c) \<Delta>\<^sub>c e) 
-      (SE\<^sub>c (tail_expr \<Delta>\<^sub>c e @ FApp2\<^sub>c c # s\<^sub>c) \<Delta>\<^sub>c (head_expr e))" by simp
-    moreover have "SC\<^sub>c (FApp1\<^sub>c \<Delta>\<^sub>c e # s\<^sub>c) c \<leadsto>\<^sub>c SE\<^sub>c (FApp2\<^sub>c c # s\<^sub>c) \<Delta>\<^sub>c e" by simp
-    moreover have "SE\<^sub>c (tail_expr \<Delta>\<^sub>c e @ FApp2\<^sub>c c # s\<^sub>c) \<Delta>\<^sub>c (Const\<^sub>d n) \<leadsto>\<^sub>c 
-      SC\<^sub>c (tail_expr \<Delta>\<^sub>c e @ FApp2\<^sub>c c # s\<^sub>c) (Const\<^sub>c n)" by simp
-    ultimately have "iter (\<leadsto>\<^sub>c) (SC\<^sub>c (FApp1\<^sub>c \<Delta>\<^sub>c e # s\<^sub>c) c)
-      (SC\<^sub>c (tail_expr \<Delta>\<^sub>c e @ FApp2\<^sub>c c # s\<^sub>c) (Const\<^sub>c n))" 
+    case (SC\<^sub>g s\<^sub>g c \<Delta>\<^sub>g e \<C>')
+    moreover have "iter (\<leadsto>\<^sub>g) (SE\<^sub>g (FApp2\<^sub>g c # s\<^sub>g) \<Delta>\<^sub>g e) 
+      (SE\<^sub>g (tail_expr \<Delta>\<^sub>g e @ FApp2\<^sub>g c # s\<^sub>g) \<Delta>\<^sub>g (head_expr e))" by simp
+    moreover have "SC\<^sub>g (FApp1\<^sub>g \<Delta>\<^sub>g e # s\<^sub>g) c \<leadsto>\<^sub>g SE\<^sub>g (FApp2\<^sub>g c # s\<^sub>g) \<Delta>\<^sub>g e" by simp
+    moreover have "SE\<^sub>g (tail_expr \<Delta>\<^sub>g e @ FApp2\<^sub>g c # s\<^sub>g) \<Delta>\<^sub>g (Const\<^sub>g n) \<leadsto>\<^sub>g 
+      SC\<^sub>g (tail_expr \<Delta>\<^sub>g e @ FApp2\<^sub>g c # s\<^sub>g) (Num\<^sub>g n)" by simp
+    ultimately have "iter (\<leadsto>\<^sub>g) (SC\<^sub>g (FApp1\<^sub>g \<Delta>\<^sub>g e # s\<^sub>g) c)
+      (SC\<^sub>g (tail_expr \<Delta>\<^sub>g e @ FApp2\<^sub>g c # s\<^sub>g) (Num\<^sub>g n))" 
         by (metis iter_step iter_step_after)
-    with SC\<^sub>c show ?case by auto
+    with SC\<^sub>g show ?case by auto
   qed
 next
   case (ev\<^sub>e_pushlam \<V> \<Delta>\<^sub>e \<C>' n \<C> s\<^sub>e)
-  hence X: "encode_state \<Sigma>\<^sub>c = S\<^sub>e \<V> ((\<Delta>\<^sub>e, PushLam\<^sub>e \<C>' n # \<C>) # s\<^sub>e)" by simp
+  hence X: "encode_state \<Sigma>\<^sub>g = S\<^sub>e \<V> ((\<Delta>\<^sub>e, PushLam\<^sub>e \<C>' n # \<C>) # s\<^sub>e)" by simp
   from X ev\<^sub>e_pushlam(2) show ?case
   proof (induction rule: encode_state_to_pushlam)
-    case (SE\<^sub>c s\<^sub>c \<Delta>\<^sub>c e tt e' \<C>'')
-    moreover have "iter (\<leadsto>\<^sub>c) (SE\<^sub>c s\<^sub>c \<Delta>\<^sub>c e) (SE\<^sub>c (tail_expr \<Delta>\<^sub>c e @ s\<^sub>c) \<Delta>\<^sub>c (head_expr e))" by simp
-    moreover have "SE\<^sub>c (tail_expr \<Delta>\<^sub>c e @ s\<^sub>c) \<Delta>\<^sub>c (Lam\<^sub>d tt e') \<leadsto>\<^sub>c 
-      SC\<^sub>c (tail_expr \<Delta>\<^sub>c e @ s\<^sub>c) (Lam\<^sub>c tt \<Delta>\<^sub>c e')" by simp
-    ultimately have E: "iter (\<leadsto>\<^sub>c) (SE\<^sub>c s\<^sub>c \<Delta>\<^sub>c e) (SC\<^sub>c (tail_expr \<Delta>\<^sub>c e @ s\<^sub>c) (Lam\<^sub>c tt \<Delta>\<^sub>c e'))"
+    case (SE\<^sub>g s\<^sub>g \<Delta>\<^sub>g e tt e' \<C>'')
+    moreover have "iter (\<leadsto>\<^sub>g) (SE\<^sub>g s\<^sub>g \<Delta>\<^sub>g e) (SE\<^sub>g (tail_expr \<Delta>\<^sub>g e @ s\<^sub>g) \<Delta>\<^sub>g (head_expr e))" by simp
+    moreover have "SE\<^sub>g (tail_expr \<Delta>\<^sub>g e @ s\<^sub>g) \<Delta>\<^sub>g (Lam\<^sub>g tt e' n) \<leadsto>\<^sub>g 
+      SC\<^sub>g (tail_expr \<Delta>\<^sub>g e @ s\<^sub>g) (Fun\<^sub>g tt \<Delta>\<^sub>g e' n)" by simp
+    ultimately have E: "iter (\<leadsto>\<^sub>g) (SE\<^sub>g s\<^sub>g \<Delta>\<^sub>g e) (SC\<^sub>g (tail_expr \<Delta>\<^sub>g e @ s\<^sub>g) (Fun\<^sub>g tt \<Delta>\<^sub>g e' n))"
       by (metis iter_step_after)
-    from SE\<^sub>c have "\<Delta>\<^sub>e = map encode_closure \<Delta>\<^sub>c" by fastforce
-    with SE\<^sub>c E show ?case by auto
+    from SE\<^sub>g have "\<Delta>\<^sub>e = map (map encode_closure) \<Delta>\<^sub>g" by fastforce
+    with SE\<^sub>g E show ?case by auto
   next
-    case (SC\<^sub>c s\<^sub>c c \<Delta>\<^sub>c e tt e' \<C>'')
-    moreover have "iter (\<leadsto>\<^sub>c) (SE\<^sub>c (FApp2\<^sub>c c # s\<^sub>c) \<Delta>\<^sub>c e) 
-      (SE\<^sub>c (tail_expr \<Delta>\<^sub>c e @ FApp2\<^sub>c c # s\<^sub>c) \<Delta>\<^sub>c (head_expr e))" by simp
-    moreover have "SC\<^sub>c (FApp1\<^sub>c \<Delta>\<^sub>c e # s\<^sub>c) c \<leadsto>\<^sub>c SE\<^sub>c (FApp2\<^sub>c c # s\<^sub>c) \<Delta>\<^sub>c e" by simp
-    moreover have "SE\<^sub>c (tail_expr \<Delta>\<^sub>c e @ FApp2\<^sub>c c # s\<^sub>c) \<Delta>\<^sub>c (Lam\<^sub>d tt e') \<leadsto>\<^sub>c 
-      SC\<^sub>c (tail_expr \<Delta>\<^sub>c e @ FApp2\<^sub>c c # s\<^sub>c) (Lam\<^sub>c tt \<Delta>\<^sub>c e')" by simp
-    ultimately have E: "iter (\<leadsto>\<^sub>c) (SC\<^sub>c (FApp1\<^sub>c \<Delta>\<^sub>c e # s\<^sub>c) c) 
-      (SC\<^sub>c (tail_expr \<Delta>\<^sub>c e @ FApp2\<^sub>c c # s\<^sub>c) (Lam\<^sub>c tt \<Delta>\<^sub>c e'))" 
+    case (SC\<^sub>g s\<^sub>g c \<Delta>\<^sub>g e tt e' \<C>'')
+    moreover have "iter (\<leadsto>\<^sub>g) (SE\<^sub>g (FApp2\<^sub>g c # s\<^sub>g) \<Delta>\<^sub>g e) 
+      (SE\<^sub>g (tail_expr \<Delta>\<^sub>g e @ FApp2\<^sub>g c # s\<^sub>g) \<Delta>\<^sub>g (head_expr e))" by simp
+    moreover have "SC\<^sub>g (FApp1\<^sub>g \<Delta>\<^sub>g e # s\<^sub>g) c \<leadsto>\<^sub>g SE\<^sub>g (FApp2\<^sub>g c # s\<^sub>g) \<Delta>\<^sub>g e" by simp
+    moreover have "SE\<^sub>g (tail_expr \<Delta>\<^sub>g e @ FApp2\<^sub>g c # s\<^sub>g) \<Delta>\<^sub>g (Lam\<^sub>g tt e' n) \<leadsto>\<^sub>g 
+      SC\<^sub>g (tail_expr \<Delta>\<^sub>g e @ FApp2\<^sub>g c # s\<^sub>g) (Fun\<^sub>g tt \<Delta>\<^sub>g e' n)" by simp
+    ultimately have E: "iter (\<leadsto>\<^sub>g) (SC\<^sub>g (FApp1\<^sub>g \<Delta>\<^sub>g e # s\<^sub>g) c) 
+      (SC\<^sub>g (tail_expr \<Delta>\<^sub>g e @ FApp2\<^sub>g c # s\<^sub>g) (Fun\<^sub>g tt \<Delta>\<^sub>g e' n))" 
         by (metis iter_step iter_step_after)
-    from SC\<^sub>c have "\<Delta>\<^sub>e = map encode_closure \<Delta>\<^sub>c" by fastforce
-    with SC\<^sub>c E show ?case by auto
+    from SC\<^sub>g have "\<Delta>\<^sub>e = map (map encode_closure) \<Delta>\<^sub>g" by fastforce
+    with SC\<^sub>g E show ?case by auto
   qed
 next
-  case (ev\<^sub>e_apply v \<Delta>\<^sub>e' \<C>' \<V> \<Delta>\<^sub>e \<C> s\<^sub>e)
-  hence "encode_state \<Sigma>\<^sub>c = S\<^sub>e (v # Lam\<^sub>e \<Delta>\<^sub>e' \<C>' # \<V>) ((\<Delta>\<^sub>e, Apply\<^sub>e # \<C>) # s\<^sub>e)" by simp
-  then obtain s\<^sub>c c c' where "\<Sigma>\<^sub>c = SC\<^sub>c (FApp2\<^sub>c c' # s\<^sub>c) c \<and> 
-    stack_from_stack s\<^sub>c = ((\<Delta>\<^sub>e, \<C>) # s\<^sub>e) \<and> v = encode_closure c \<and> 
-    Lam\<^sub>e \<Delta>\<^sub>e' \<C>' = encode_closure c' \<and> \<V> = vals_from_stack s\<^sub>c" 
+  case (ev\<^sub>e_apply v \<Delta>\<^sub>e' \<C>' n \<V> \<Delta>\<^sub>e \<C> s\<^sub>e)
+  hence "encode_state \<Sigma>\<^sub>g = S\<^sub>e (v # Lam\<^sub>e \<Delta>\<^sub>e' \<C>' n # \<V>) ((\<Delta>\<^sub>e, Apply\<^sub>e # \<C>) # s\<^sub>e)" by simp
+  then obtain s\<^sub>g c c' where "\<Sigma>\<^sub>g = SC\<^sub>g (FApp2\<^sub>g c' # s\<^sub>g) c \<and> 
+    stack_from_stack s\<^sub>g = ((\<Delta>\<^sub>e, \<C>) # s\<^sub>e) \<and> v = encode_closure c \<and> 
+    Lam\<^sub>e \<Delta>\<^sub>e' \<C>' n = encode_closure c' \<and> \<V> = vals_from_stack s\<^sub>g" 
       by auto
-  moreover then obtain t \<Delta>\<^sub>c e where "c' = Lam\<^sub>c t \<Delta>\<^sub>c e \<and> \<Delta>\<^sub>e' = map encode_closure \<Delta>\<^sub>c \<and> 
+  moreover then obtain t \<Delta>\<^sub>g e where "c' = Fun\<^sub>g t \<Delta>\<^sub>g e n \<and> \<Delta>\<^sub>e' = map (map encode_closure) \<Delta>\<^sub>g \<and> 
     \<C>' = encode e" by auto
-  moreover have "SC\<^sub>c (FApp2\<^sub>c (Lam\<^sub>c t \<Delta>\<^sub>c e) # s\<^sub>c) c \<leadsto>\<^sub>c SE\<^sub>c (FReturn\<^sub>c (c # \<Delta>\<^sub>c) # s\<^sub>c) (c # \<Delta>\<^sub>c) e" 
+  moreover have "SC\<^sub>g (FApp2\<^sub>g (Fun\<^sub>g t \<Delta>\<^sub>g e n) # s\<^sub>g) c \<leadsto>\<^sub>g SE\<^sub>g (FReturn\<^sub>g ([c] # \<Delta>\<^sub>g) # s\<^sub>g) ([c] # \<Delta>\<^sub>g) e" 
     by simp
-  moreover hence "iter (\<leadsto>\<^sub>c) (SC\<^sub>c (FApp2\<^sub>c (Lam\<^sub>c t \<Delta>\<^sub>c e) # s\<^sub>c) c) 
-    (SE\<^sub>c (FReturn\<^sub>c (c # \<Delta>\<^sub>c) # s\<^sub>c) (c # \<Delta>\<^sub>c) e)" by (metis iter_one)
+  moreover hence "iter (\<leadsto>\<^sub>g) (SC\<^sub>g (FApp2\<^sub>g (Fun\<^sub>g t \<Delta>\<^sub>g e n) # s\<^sub>g) c) 
+    (SE\<^sub>g (FReturn\<^sub>g ([c] # \<Delta>\<^sub>g) # s\<^sub>g) ([c] # \<Delta>\<^sub>g) e)" by (metis iter_one)
   ultimately show ?case by (auto simp add: encode_def)
 next
   case (ev\<^sub>e_pushenv v \<V> \<Delta>\<^sub>e \<C> s\<^sub>e)
-  hence "encode_state \<Sigma>\<^sub>c = S\<^sub>e (v # \<V>) ((\<Delta>\<^sub>e, PushEnv\<^sub>e # \<C>) # s\<^sub>e)" by simp
-  then obtain c s\<^sub>c where S: "\<Sigma>\<^sub>c = SC\<^sub>c s\<^sub>c c \<and> v = encode_closure c \<and> \<V> = vals_from_stack s\<^sub>c \<and> 
-    stack_from_stack s\<^sub>c = (\<Delta>\<^sub>e, PushEnv\<^sub>e # \<C>) # s\<^sub>e" by auto
-  then obtain s\<^sub>c' \<Delta>\<^sub>c e \<C>' where S':  "s\<^sub>c = FLet\<^sub>c \<Delta>\<^sub>c e # s\<^sub>c' \<and> \<C> = encode' e @ PopEnv\<^sub>e # \<C>' \<and> 
-    stack_from_stack s\<^sub>c' = (\<Delta>\<^sub>e, \<C>') # s\<^sub>e" by auto
-  have "SC\<^sub>c (FLet\<^sub>c \<Delta>\<^sub>c e # s\<^sub>c') c \<leadsto>\<^sub>c SE\<^sub>c (FPop\<^sub>c c # s\<^sub>c') (c # \<Delta>\<^sub>c) e" by simp
-  hence "iter (\<leadsto>\<^sub>c) (SC\<^sub>c (FLet\<^sub>c \<Delta>\<^sub>c e # s\<^sub>c') c) (SE\<^sub>c (FPop\<^sub>c c # s\<^sub>c') (c # \<Delta>\<^sub>c) e)" 
+  hence "encode_state \<Sigma>\<^sub>g = S\<^sub>e (v # \<V>) ((\<Delta>\<^sub>e, PushEnv\<^sub>e # \<C>) # s\<^sub>e)" by simp
+  then obtain c s\<^sub>g where S: "\<Sigma>\<^sub>g = SC\<^sub>g s\<^sub>g c \<and> v = encode_closure c \<and> \<V> = vals_from_stack s\<^sub>g \<and> 
+    stack_from_stack s\<^sub>g = (\<Delta>\<^sub>e, PushEnv\<^sub>e # \<C>) # s\<^sub>e" by auto
+  then obtain s\<^sub>g' \<Delta>\<^sub>g e \<C>' where S':  "s\<^sub>g = FLet\<^sub>g \<Delta>\<^sub>g e # s\<^sub>g' \<and> \<C> = encode' e @ PopEnv\<^sub>e # \<C>' \<and> 
+    stack_from_stack s\<^sub>g' = (\<Delta>\<^sub>e, \<C>') # s\<^sub>e" by auto
+  have "SC\<^sub>g (FLet\<^sub>g \<Delta>\<^sub>g e # s\<^sub>g') c \<leadsto>\<^sub>g SE\<^sub>g (FPop\<^sub>g c # s\<^sub>g') (cons_fst c \<Delta>\<^sub>g) e" by simp
+  hence "iter (\<leadsto>\<^sub>g) (SC\<^sub>g (FLet\<^sub>g \<Delta>\<^sub>g e # s\<^sub>g') c) (SE\<^sub>g (FPop\<^sub>g c # s\<^sub>g') (cons_fst c \<Delta>\<^sub>g) e)" 
     by (metis iter_one)
   with S S' show ?case by auto
 next
-  case (ev\<^sub>e_popenv \<V> v \<Delta>\<^sub>e \<C> s\<^sub>e)
-  hence "encode_state \<Sigma>\<^sub>c = S\<^sub>e \<V> ((v # \<Delta>\<^sub>e, PopEnv\<^sub>e # \<C>) # s\<^sub>e)" by simp
-  then obtain c s\<^sub>c where S: "\<Sigma>\<^sub>c = SC\<^sub>c s\<^sub>c c \<and> \<V> = encode_closure c # vals_from_stack s\<^sub>c \<and> 
-    stack_from_stack s\<^sub>c = (v # \<Delta>\<^sub>e, PopEnv\<^sub>e # \<C>) # s\<^sub>e" by auto
-  then obtain s\<^sub>c' c' \<Delta>\<^sub>e' where S': "s\<^sub>c = FPop\<^sub>c c' # s\<^sub>c' \<and> v # \<Delta>\<^sub>e = encode_closure c' # \<Delta>\<^sub>e' \<and> 
-    stack_from_stack s\<^sub>c' = (\<Delta>\<^sub>e', \<C>) # s\<^sub>e" by auto
-  have "SC\<^sub>c (FPop\<^sub>c c' # s\<^sub>c') c \<leadsto>\<^sub>c SC\<^sub>c s\<^sub>c' c" by simp
-  hence "iter (\<leadsto>\<^sub>c) (SC\<^sub>c (FPop\<^sub>c c' # s\<^sub>c') c) (SC\<^sub>c s\<^sub>c' c)" by (metis iter_one)
-  with S S' show ?case by auto
+  case (ev\<^sub>e_popenv \<V> v vs \<Delta>\<^sub>e \<C> s\<^sub>e)
+  hence "encode_state \<Sigma>\<^sub>g = S\<^sub>e \<V> (((v # vs) # \<Delta>\<^sub>e, PopEnv\<^sub>e # \<C>) # s\<^sub>e)" by simp
+  then obtain c s\<^sub>g where S: "\<Sigma>\<^sub>g = SC\<^sub>g s\<^sub>g c \<and> \<V> = encode_closure c # vals_from_stack s\<^sub>g \<and> 
+    stack_from_stack s\<^sub>g = ((v # vs) # \<Delta>\<^sub>e, PopEnv\<^sub>e # \<C>) # s\<^sub>e" by auto
+  then obtain s\<^sub>g' c' \<Delta>\<^sub>e' where S': "s\<^sub>g = FPop\<^sub>g c' # s\<^sub>g' \<and> 
+    (v # vs) # \<Delta>\<^sub>e = (encode_closure c' # vs) # \<Delta>\<^sub>e' \<and> stack_from_stack s\<^sub>g' = (\<Delta>\<^sub>e', \<C>) # s\<^sub>e" 
+      by auto
+  have "SC\<^sub>g (FPop\<^sub>g c' # s\<^sub>g') c \<leadsto>\<^sub>g SC\<^sub>g s\<^sub>g' c" by simp
+  hence "iter (\<leadsto>\<^sub>g) (SC\<^sub>g (FPop\<^sub>g c' # s\<^sub>g') c) (SC\<^sub>g s\<^sub>g' c)" by (metis iter_one)
+  with ev\<^sub>e_popenv S S' show ?case by auto
 next
   case (ev\<^sub>e_return \<V> \<Delta>\<^sub>e \<C> s\<^sub>e)
-  hence "encode_state \<Sigma>\<^sub>c = S\<^sub>e \<V> ((\<Delta>\<^sub>e, Return\<^sub>e # \<C>) # s\<^sub>e)" by simp
-  then obtain \<Delta>\<^sub>c s\<^sub>c c where S: "\<Sigma>\<^sub>c = SC\<^sub>c (FReturn\<^sub>c \<Delta>\<^sub>c # s\<^sub>c) c \<and> s\<^sub>e = stack_from_stack s\<^sub>c \<and>
-    \<Delta>\<^sub>e = map encode_closure \<Delta>\<^sub>c \<and> \<V> = encode_closure c # vals_from_stack s\<^sub>c" by auto
-  have "SC\<^sub>c (FReturn\<^sub>c \<Delta>\<^sub>c # s\<^sub>c) c \<leadsto>\<^sub>c SC\<^sub>c s\<^sub>c c" by simp
-  hence "iter (\<leadsto>\<^sub>c) (SC\<^sub>c (FReturn\<^sub>c \<Delta>\<^sub>c # s\<^sub>c) c) (SC\<^sub>c s\<^sub>c c)" by (metis iter_one)
+  hence "encode_state \<Sigma>\<^sub>g = S\<^sub>e \<V> ((\<Delta>\<^sub>e, Return\<^sub>e # \<C>) # s\<^sub>e)" by simp
+  then obtain \<Delta>\<^sub>g s\<^sub>g c where S: "\<Sigma>\<^sub>g = SC\<^sub>g (FReturn\<^sub>g \<Delta>\<^sub>g # s\<^sub>g) c \<and> s\<^sub>e = stack_from_stack s\<^sub>g \<and>
+    \<Delta>\<^sub>e = map (map encode_closure) \<Delta>\<^sub>g \<and> \<V> = encode_closure c # vals_from_stack s\<^sub>g" by auto
+  have "SC\<^sub>g (FReturn\<^sub>g \<Delta>\<^sub>g # s\<^sub>g) c \<leadsto>\<^sub>g SC\<^sub>g s\<^sub>g c" by simp
+  hence "iter (\<leadsto>\<^sub>g) (SC\<^sub>g (FReturn\<^sub>g \<Delta>\<^sub>g # s\<^sub>g) c) (SC\<^sub>g s\<^sub>g c)" by (metis iter_one)
   with S show ?case by auto
 next
-  case (ev\<^sub>e_jump v \<Delta>\<^sub>e' \<C>' \<V> \<Delta>\<^sub>e \<C> s\<^sub>e)
-  hence "encode_state \<Sigma>\<^sub>c = S\<^sub>e (v # Lam\<^sub>e \<Delta>\<^sub>e' \<C>' # \<V>) ((\<Delta>\<^sub>e, Jump\<^sub>e # \<C>) # s\<^sub>e)" by simp
+  case (ev\<^sub>e_jump v \<Delta>\<^sub>e' \<C>' n \<V> \<Delta>\<^sub>e \<C> s\<^sub>e)
+  hence "encode_state \<Sigma>\<^sub>g = S\<^sub>e (v # Lam\<^sub>e \<Delta>\<^sub>e' \<C>' n # \<V>) ((\<Delta>\<^sub>e, Jump\<^sub>e # \<C>) # s\<^sub>e)" by simp
   thus ?case by auto
 qed
 
